format-version: 1.2
data-version: releases/2025-03-28
idspace: dce http://purl.org/dc/elements/1.1/ 
idspace: dcterms http://purl.org/dc/terms/ 
ontology: sudo
property_value: dcterms:description "None" xsd:string
property_value: dcterms:license https://creativecommons.org/licenses/unspecified
property_value: dcterms:title "Substance Use Diagnosis Ontology" xsd:string
property_value: owl:versionInfo "2025-03-28" xsd:string

[Term]
id: 000001
name: substance use phenotype
property_value: dcterms:description "An observable state that is characterizing the use, or lack thereof, of a chemical compound with psychoactive properties." xsd:string

[Term]
id: 000002
name: substance use
is_a: 000001 ! substance use phenotype
property_value: dcterms:description "A substance use phenotype in which a substance is used. Use may be through inhalation, injection, ingestion or other means by which the substance may enter the body." xsd:string

[Term]
id: 000003
name: no known substance use
is_a: 000001 ! substance use phenotype
property_value: dcterms:description "A type of substance use phenotype in which there is no knowledge or evidence for any use of a substance." xsd:string

[Term]
id: 000004
name: no known substance use disorder
is_a: 000003 ! no known substance use
property_value: dcterms:description "A type of substance use phenotype in which there is no knowledge or evidence for a substance use disorder." xsd:string

[Term]
id: 000005
name: no known active substance use
is_a: 000001 ! substance use phenotype
property_value: dcterms:description "A type of substance use phenotype in which there has been substance use in the past, but there is no evidence or knowledge of any current substance use." xsd:string

[Term]
id: 000006
name: non-repetitive binge substance use
is_a: 000002 ! substance use
property_value: dcterms:description "A type of substance use characterized by isolated or sporadic use of significant quantities of a substance in a short time period." xsd:string

[Term]
id: 000007
name: recreational substance use
is_a: 000002 ! substance use
property_value: dcterms:description "A type of substance use characterized by occasional limited use of a substance, without adverse consequences or behavioral/physiologic symptoms of a substance use disorder." xsd:string

[Term]
id: 000008
name: chronic substance use
is_a: 000002 ! substance use
property_value: dcterms:description "A type of substance use in which the use of the substance is frequent and persistent for a period of 3 months or greater; may or may not be accompanied by behavioral or physiologic symptoms necessary to define a substance use disorder." xsd:string

[Term]
id: 000009
name: alcohol use
is_a: 000002 ! substance use
property_value: dcterms:description "A substance use phenotype in which alcohol is used. Use may be through inhalation, injection, ingestion or other means by which the substance may enter the body." xsd:string

[Term]
id: 000010
name: non-repetitive binge alcohol use
is_a: 000006 ! non-repetitive binge substance use
is_a: 000009 ! alcohol use
property_value: dcterms:description "A type of alcohol use characterized by isolated or sporadic use of significant quantities of alcohol in a short time period." xsd:string

[Term]
id: 000011
name: recreational alcohol use
is_a: 000007 ! recreational substance use
is_a: 000009 ! alcohol use
property_value: dcterms:description "A type of alcohol use characterized by occasional limited use of alcohol, without adverse consequences or behavioral/physiologic symptoms of a substance use disorder." xsd:string

[Term]
id: 000012
name: chronic alcohol use
is_a: 000008 ! chronic substance use
is_a: 000009 ! alcohol use
property_value: dcterms:description "A type of alcohol use in which the use of alcohol is frequent and persistent for a period of 3 months or greater; may or may not be accompanied by behavioral or physiologic symptoms necessary to define a substance use disorder." xsd:string

[Term]
id: 000013
name: alcohol use disorder
is_a: 000012 ! chronic alcohol use
property_value: dcterms:description "A type of chronic alcohol use where there is continued use of alcohol despite harm or adverse consequence to self or others. This is defined by behavioral criteria and physiologic symptoms." xsd:string

[Term]
id: 000014
name: alcohol abuse
is_a: 000013 ! alcohol use disorder
property_value: dcterms:description "A type of alcohol use in which the amounts or methods of use of alcohol are harmful or problematic to the individual or others (also called alcohol misuse)" xsd:string

[Term]
id: 000015
name: DSM_IV-defined subsyndromic alcohol abuse
is_a: 000014 ! alcohol abuse
property_value: isDefinedBy "DSM_IV" xsd:string

[Term]
id: 000016
name: DSM_IV-defined syndromic alcohol abuse
is_a: 000014 ! alcohol abuse
property_value: dcterms:description "A maladaptive pattern of alcohol use leading to clinically significant impairment or distress, as manifested by one (or more) of the following, occurring within a 12-month period: 1) Recurrent alcohol use resulting in a failure to fulfill major role obligation at work, school, or home; 2) Recurrent alcohol use in situations in which it is physically hazardous; 3) Recurrent alcohol-related legal problems; 4) Continued alcohol use despite having persistent or recurrent social or interpersonal problems caused or exacerbated by the effects of alcohol." xsd:string
property_value: isDefinedBy "DSM_IV" xsd:string

[Term]
id: 000017
name: alcohol dependence
is_a: 000013 ! alcohol use disorder
property_value: dcterms:description "A type of alcohol use in which the use of alcohol is compulsive and repetitive and may result in tolerance to the effect of the drug and withdrawal symptoms when use is reduced or stopped." xsd:string

[Term]
id: 000018
name: DSM_IV-defined subsyndromic alcohol dependence
is_a: 000017 ! alcohol dependence
property_value: dcterms:description "A pattern of alcohol use, leading to impairment or distress, as manifested by one to two of the following, occurring at any time in the same 12-month period: 1) Tolerance, as defined by either the following: a. Need for markedly increased amounts of alcohol to achieve intoxication or desired effect. b. Markedly diminished effect with continued use of the same amount of alcohol; 2) Withdrawal, as manifested by either of the following: a. The characteristic withdrawal syndrome for alcohol. b. The same (or closely related) substance is taken to relieve or avoid withdrawal symptoms; 3) alcohol is often taken in larger amounts or over a longer period than was intended; 4) There is persistent desire or unsuccessful efforts to cut down or control alcohol use; 5) A great deal of time is spent in activities necessary to obtain alcohol, use alcohol or recover from its effects; 6) Important social, occupational, or recreational activities are given up or reduced because of alcohol use; 7) alcohol use is continued despite knowledge of having a persistent or recurrent physical or psychological problem that is likely to have been caused or exacerbated by alcohol." xsd:string
property_value: isDefinedBy "DSM_IV" xsd:string

[Term]
id: 000019
name: DSM_IV-defined syndromic alcohol dependence
is_a: 000017 ! alcohol dependence
property_value: dcterms:description "A maladaptive pattern of alcohol use, leading to significant impairment or distress, as manifested by three (or more) of the following, occurring at any time in the same 12-month period: 1) Tolerance, as defined by either the following: a. Need for markedly increased amounts of alcohol to achieve intoxication or desired effect. b. Markedly diminished effect with continued use of the same amount of alcohol; 2) Withdrawal, as manifested by either of the following: a. The characteristic withdrawal syndrome for alcohol. b. The same (or closely related) substance is taken to relieve or avoid withdrawal symptoms; 3) alcohol is often taken in larger amounts or over a longer period than was intended; 4) There is persistent desire or unsuccessful efforts to cut down or control alcohol use; 5) A great deal of time is spent in activities necessary to obtain alcohol, use alcohol or recover from its effects; 6) Important social, occupational, or recreational activities are given up or reduced because of alcohol use; 7) alcohol use is continued despite knowledge of having a persistent or recurrent physical or psychological problem that is likely to have been caused or exacerbated by alcohol." xsd:string
property_value: isDefinedBy "DSM_IV" xsd:string

[Term]
id: 000020
name: DSM_V-defined mild alcohol use disorder
is_a: 000013 ! alcohol use disorder
property_value: dcterms:description "A problematic pattern of alcohol use leading to clinically significant impairment or distress, as manifested by two of the following, occurring within a 12-month period: 1) alcohol is often taken in larger amounts or over a longer period than was intended; 2) There is a persistent desire or unsuccessful efforts to cut down or control alcohol use; 3) A great deal of time is spent in activities necessary to obtain alcohol, use alcohol, or recover from its effects; 4) Craving, or a strong desire or urge to use alcohol; 5) Recurrent alcohol use resulting in a failure to fulfill major role obligations at work, school, or home; 6) Continued alcohol use despite having persistent or recurrent social or interpersonal problems caused or exacerbated by the effects of alcohol; 7) Important social, occupational, or recreational activities are given up or reduced because of alcohol use; 8) Recurrent alcohol use in situations in which it is physically hazardous; 9) alcohol use is continued despite knowledge of having a persistent or recurrent physical or psychological problem that is likely to have been caused or exacerbated by alcohol; 10) Tolerance, as defined by either of the following:a. A need for markedly increased amounts of alcohol to achieve intoxication or desired effect b. A markedly diminished effect with continued use of the same amount of alcohol; 11) Withdrawal, as manifested by either of the following: a. The characteristic withdrawal syndrome for alcohol. b. alcohol (or a closely related substance) is taken to relieve or avoid withdrawal symptoms." xsd:string
property_value: isDefinedBy "DSM_V" xsd:string

[Term]
id: 000021
name: DSM_V-defined moderate alcohol use disorder
is_a: 000013 ! alcohol use disorder
property_value: dcterms:description "A problematic pattern of alcohol use leading to clinically significant impairment or distress, as manifested by 4-5 of the following, occurring within a 12-month period: 1) alcohol is often taken in larger amounts or over a longer period than was intended; 2) There is a persistent desire or unsuccessful efforts to cut down or control alcohol use; 3) A great deal of time is spent in activities necessary to obtain alcohol, use alcohol, or recover from its effects; 4) Craving, or a strong desire or urge to use alcohol; 5) Recurrent alcohol use resulting in a failure to fulfill major role obligations at work, school, or home; 6) Continued alcohol use despite having persistent or recurrent social or interpersonal problems caused or exacerbated by the effects of alcohol; 7) Important social, occupational, or recreational activities are given up or reduced because of alcohol use; 8) Recurrent alcohol use in situations in which it is physically hazardous; 9) alcohol use is continued despite knowledge of having a persistent or recurrent physical or psychological problem that is likely to have been caused or exacerbated by alcohol; 10) Tolerance, as defined by either of the following:a. A need for markedly increased amounts of alcohol to achieve intoxication or desired effect b. A markedly diminished effect with continued use of the same amount of alcohol; 11) Withdrawal, as manifested by either of the following: a. The characteristic withdrawal syndrome for alcohol. b. alcohol (or a closely related substance) is taken to relieve or avoid withdrawal symptoms." xsd:string
property_value: isDefinedBy "DSM_V" xsd:string

[Term]
id: 000022
name: DSM_V-defined severe alcohol use disorder
is_a: 000013 ! alcohol use disorder
property_value: dcterms:description "A problematic pattern of alcohol use leading to clinically significant impairment or distress, as manifested by six or more of the following, occurring within a 12-month period: 1) alcohol is often taken in larger amounts or over a longer period than was intended; 2) There is a persistent desire or unsuccessful efforts to cut down or control alcohol use; 3) A great deal of time is spent in activities necessary to obtain alcohol, use alcohol, or recover from its effects; 4) Craving, or a strong desire or urge to use alcohol; 5) Recurrent alcohol use resulting in a failure to fulfill major role obligations at work, school, or home; 6) Continued alcohol use despite having persistent or recurrent social or interpersonal problems caused or exacerbated by the effects of alcohol; 7) Important social, occupational, or recreational activities are given up or reduced because of alcohol use; 8) Recurrent alcohol use in situations in which it is physically hazardous; 9) alcohol use is continued despite knowledge of having a persistent or recurrent physical or psychological problem that is likely to have been caused or exacerbated by alcohol; 10) Tolerance, as defined by either of the following:a. A need for markedly increased amounts of alcohol to achieve intoxication or desired effect b. A markedly diminished effect with continued use of the same amount of alcohol; 11) Withdrawal, as manifested by either of the following: a. The characteristic withdrawal syndrome for alcohol. b. alcohol (or a closely related substance) is taken to relieve or avoid withdrawal symptoms." xsd:string
property_value: isDefinedBy "DSM_V" xsd:string

[Term]
id: 000023
name: cannabis use
is_a: 000002 ! substance use
property_value: dcterms:description "A substance use phenotype in which cannabis is used. Use may be through inhalation, injection, ingestion or other means by which the substance may enter the body." xsd:string

[Term]
id: 000024
name: non-repetitive binge cannabis use
is_a: 000006 ! non-repetitive binge substance use
is_a: 000023 ! cannabis use
property_value: dcterms:description "A type of cannabis use characterized by isolated or sporadic use of significant quantities of cannabis in a short time period." xsd:string

[Term]
id: 000025
name: recreational cannabis use
is_a: 000007 ! recreational substance use
is_a: 000023 ! cannabis use
property_value: dcterms:description "A type of cannabis use characterized by occasional limited use of cannabis, without adverse consequences or behavioral/physiologic symptoms of a substance use disorder." xsd:string

[Term]
id: 000026
name: chronic cannabis use
is_a: 000008 ! chronic substance use
is_a: 000023 ! cannabis use
property_value: dcterms:description "A type of cannabis use in which the use of cannabis is frequent and persistent for a period of 3 months or greater; may or may not be accompanied by behavioral or physiologic symptoms necessary to define a substance use disorder." xsd:string

[Term]
id: 000027
name: cannabis use disorder
is_a: 000026 ! chronic cannabis use
property_value: dcterms:description "A type of chronic cannabis use where there is continued use of cannabis despite harm or adverse consequence to self or others. This is defined by behavioral criteria and physiologic symptoms." xsd:string

[Term]
id: 000028
name: cannabis abuse
is_a: 000027 ! cannabis use disorder
property_value: dcterms:description "A type of cannabis use in which the amounts or methods of use of cannabis are harmful or problematic to the individual or others (also called cannabis misuse)" xsd:string

[Term]
id: 000029
name: DSM_IV-defined subsyndromic cannabis abuse
is_a: 000028 ! cannabis abuse
property_value: isDefinedBy "DSM_IV" xsd:string

[Term]
id: 000030
name: DSM_IV-defined syndromic cannabis abuse
is_a: 000028 ! cannabis abuse
property_value: dcterms:description "A maladaptive pattern of cannabis use leading to clinically significant impairment or distress, as manifested by one (or more) of the following, occurring within a 12-month period: 1) Recurrent cannabis use resulting in a failure to fulfill major role obligation at work, school, or home; 2) Recurrent cannabis use in situations in which it is physically hazardous; 3) Recurrent cannabis-related legal problems; 4) Continued cannabis use despite having persistent or recurrent social or interpersonal problems caused or exacerbated by the effects of cannabis." xsd:string
property_value: isDefinedBy "DSM_IV" xsd:string

[Term]
id: 000031
name: cannabis dependence
is_a: 000027 ! cannabis use disorder
property_value: dcterms:description "A type of cannabis use in which the use of cannabis is compulsive and repetitive and may result in tolerance to the effect of the drug and withdrawal symptoms when use is reduced or stopped." xsd:string

[Term]
id: 000032
name: DSM_IV-defined subsyndromic cannabis dependence
is_a: 000031 ! cannabis dependence
property_value: dcterms:description "A pattern of cannabis use, leading to impairment or distress, as manifested by one to two of the following, occurring at any time in the same 12-month period: 1) Tolerance, as defined by either the following: a. Need for markedly increased amounts of cannabis to achieve intoxication or desired effect. b. Markedly diminished effect with continued use of the same amount of cannabis; 2) Withdrawal, as manifested by either of the following: a. The characteristic withdrawal syndrome for cannabis. b. The same (or closely related) substance is taken to relieve or avoid withdrawal symptoms; 3) cannabis is often taken in larger amounts or over a longer period than was intended; 4) There is persistent desire or unsuccessful efforts to cut down or control cannabis use; 5) A great deal of time is spent in activities necessary to obtain cannabis, use cannabis or recover from its effects; 6) Important social, occupational, or recreational activities are given up or reduced because of cannabis use; 7) cannabis use is continued despite knowledge of having a persistent or recurrent physical or psychological problem that is likely to have been caused or exacerbated by cannabis." xsd:string
property_value: isDefinedBy "DSM_IV" xsd:string

[Term]
id: 000033
name: DSM_IV-defined syndromic cannabis dependence
is_a: 000031 ! cannabis dependence
property_value: dcterms:description "A maladaptive pattern of cannabis use, leading to significant impairment or distress, as manifested by three (or more) of the following, occurring at any time in the same 12-month period: 1) Tolerance, as defined by either the following: a. Need for markedly increased amounts of cannabis to achieve intoxication or desired effect. b. Markedly diminished effect with continued use of the same amount of cannabis; 2) Withdrawal, as manifested by either of the following: a. The characteristic withdrawal syndrome for cannabis. b. The same (or closely related) substance is taken to relieve or avoid withdrawal symptoms; 3) cannabis is often taken in larger amounts or over a longer period than was intended; 4) There is persistent desire or unsuccessful efforts to cut down or control cannabis use; 5) A great deal of time is spent in activities necessary to obtain cannabis, use cannabis or recover from its effects; 6) Important social, occupational, or recreational activities are given up or reduced because of cannabis use; 7) cannabis use is continued despite knowledge of having a persistent or recurrent physical or psychological problem that is likely to have been caused or exacerbated by cannabis." xsd:string
property_value: isDefinedBy "DSM_IV" xsd:string

[Term]
id: 000034
name: DSM_V-defined mild cannabis use disorder
is_a: 000027 ! cannabis use disorder
property_value: dcterms:description "A problematic pattern of cannabis use leading to clinically significant impairment or distress, as manifested by two of the following, occurring within a 12-month period: 1) cannabis is often taken in larger amounts or over a longer period than was intended; 2) There is a persistent desire or unsuccessful efforts to cut down or control cannabis use; 3) A great deal of time is spent in activities necessary to obtain cannabis, use cannabis, or recover from its effects; 4) Craving, or a strong desire or urge to use cannabis; 5) Recurrent cannabis use resulting in a failure to fulfill major role obligations at work, school, or home; 6) Continued cannabis use despite having persistent or recurrent social or interpersonal problems caused or exacerbated by the effects of cannabis; 7) Important social, occupational, or recreational activities are given up or reduced because of cannabis use; 8) Recurrent cannabis use in situations in which it is physically hazardous; 9) cannabis use is continued despite knowledge of having a persistent or recurrent physical or psychological problem that is likely to have been caused or exacerbated by cannabis; 10) Tolerance, as defined by either of the following:a. A need for markedly increased amounts of cannabis to achieve intoxication or desired effect b. A markedly diminished effect with continued use of the same amount of cannabis; 11) Withdrawal, as manifested by either of the following: a. The characteristic withdrawal syndrome for cannabis. b. cannabis (or a closely related substance) is taken to relieve or avoid withdrawal symptoms." xsd:string
property_value: isDefinedBy "DSM_V" xsd:string

[Term]
id: 000035
name: DSM_V-defined moderate cannabis use disorder
is_a: 000027 ! cannabis use disorder
property_value: dcterms:description "A problematic pattern of cannabis use leading to clinically significant impairment or distress, as manifested by 4-5 of the following, occurring within a 12-month period: 1) cannabis is often taken in larger amounts or over a longer period than was intended; 2) There is a persistent desire or unsuccessful efforts to cut down or control cannabis use; 3) A great deal of time is spent in activities necessary to obtain cannabis, use cannabis, or recover from its effects; 4) Craving, or a strong desire or urge to use cannabis; 5) Recurrent cannabis use resulting in a failure to fulfill major role obligations at work, school, or home; 6) Continued cannabis use despite having persistent or recurrent social or interpersonal problems caused or exacerbated by the effects of cannabis; 7) Important social, occupational, or recreational activities are given up or reduced because of cannabis use; 8) Recurrent cannabis use in situations in which it is physically hazardous; 9) cannabis use is continued despite knowledge of having a persistent or recurrent physical or psychological problem that is likely to have been caused or exacerbated by cannabis; 10) Tolerance, as defined by either of the following:a. A need for markedly increased amounts of cannabis to achieve intoxication or desired effect b. A markedly diminished effect with continued use of the same amount of cannabis; 11) Withdrawal, as manifested by either of the following: a. The characteristic withdrawal syndrome for cannabis. b. cannabis (or a closely related substance) is taken to relieve or avoid withdrawal symptoms." xsd:string
property_value: isDefinedBy "DSM_V" xsd:string

[Term]
id: 000036
name: DSM_V-defined severe cannabis use disorder
is_a: 000027 ! cannabis use disorder
property_value: dcterms:description "A problematic pattern of cannabis use leading to clinically significant impairment or distress, as manifested by six or more of the following, occurring within a 12-month period: 1) cannabis is often taken in larger amounts or over a longer period than was intended; 2) There is a persistent desire or unsuccessful efforts to cut down or control cannabis use; 3) A great deal of time is spent in activities necessary to obtain cannabis, use cannabis, or recover from its effects; 4) Craving, or a strong desire or urge to use cannabis; 5) Recurrent cannabis use resulting in a failure to fulfill major role obligations at work, school, or home; 6) Continued cannabis use despite having persistent or recurrent social or interpersonal problems caused or exacerbated by the effects of cannabis; 7) Important social, occupational, or recreational activities are given up or reduced because of cannabis use; 8) Recurrent cannabis use in situations in which it is physically hazardous; 9) cannabis use is continued despite knowledge of having a persistent or recurrent physical or psychological problem that is likely to have been caused or exacerbated by cannabis; 10) Tolerance, as defined by either of the following:a. A need for markedly increased amounts of cannabis to achieve intoxication or desired effect b. A markedly diminished effect with continued use of the same amount of cannabis; 11) Withdrawal, as manifested by either of the following: a. The characteristic withdrawal syndrome for cannabis. b. cannabis (or a closely related substance) is taken to relieve or avoid withdrawal symptoms." xsd:string
property_value: isDefinedBy "DSM_V" xsd:string

[Term]
id: 000037
name: hallucinogen use
is_a: 000002 ! substance use
property_value: dcterms:description "A substance use phenotype in which hallucinogen is used. Use may be through inhalation, injection, ingestion or other means by which the substance may enter the body." xsd:string

[Term]
id: 000038
name: non-repetitive binge hallucinogen use
is_a: 000006 ! non-repetitive binge substance use
is_a: 000037 ! hallucinogen use
property_value: dcterms:description "A type of hallucinogen use characterized by isolated or sporadic use of significant quantities of hallucinogen in a short time period." xsd:string

[Term]
id: 000039
name: recreational hallucinogen use
is_a: 000007 ! recreational substance use
is_a: 000037 ! hallucinogen use
property_value: dcterms:description "A type of hallucinogen use characterized by occasional limited use of hallucinogen, without adverse consequences or behavioral/physiologic symptoms of a substance use disorder." xsd:string

[Term]
id: 000040
name: chronic hallucinogen use
is_a: 000008 ! chronic substance use
is_a: 000037 ! hallucinogen use
property_value: dcterms:description "A type of hallucinogen use in which the use of hallucinogen is frequent and persistent for a period of 3 months or greater; may or may not be accompanied by behavioral or physiologic symptoms necessary to define a substance use disorder." xsd:string

[Term]
id: 000041
name: hallucinogen use disorder
is_a: 000040 ! chronic hallucinogen use
property_value: dcterms:description "A type of chronic hallucinogen use where there is continued use of hallucinogen despite harm or adverse consequence to self or others. This is defined by behavioral criteria and physiologic symptoms." xsd:string

[Term]
id: 000042
name: hallucinogen abuse
is_a: 000041 ! hallucinogen use disorder
property_value: dcterms:description "A type of hallucinogen use in which the amounts or methods of use of hallucinogen are harmful or problematic to the individual or others (also called hallucinogen misuse)" xsd:string

[Term]
id: 000043
name: DSM_IV-defined subsyndromic hallucinogen abuse
is_a: 000042 ! hallucinogen abuse
property_value: isDefinedBy "DSM_IV" xsd:string

[Term]
id: 000044
name: DSM_IV-defined syndromic hallucinogen abuse
is_a: 000042 ! hallucinogen abuse
property_value: dcterms:description "A maladaptive pattern of hallucinogen use leading to clinically significant impairment or distress, as manifested by one (or more) of the following, occurring within a 12-month period: 1) Recurrent hallucinogen use resulting in a failure to fulfill major role obligation at work, school, or home; 2) Recurrent hallucinogen use in situations in which it is physically hazardous; 3) Recurrent hallucinogen-related legal problems; 4) Continued hallucinogen use despite having persistent or recurrent social or interpersonal problems caused or exacerbated by the effects of hallucinogen." xsd:string
property_value: isDefinedBy "DSM_IV" xsd:string

[Term]
id: 000045
name: hallucinogen dependence
is_a: 000041 ! hallucinogen use disorder
property_value: dcterms:description "A type of hallucinogen use in which the use of hallucinogen is compulsive and repetitive and may result in tolerance to the effect of the drug and withdrawal symptoms when use is reduced or stopped." xsd:string

[Term]
id: 000046
name: DSM_IV-defined subsyndromic hallucinogen dependence
is_a: 000045 ! hallucinogen dependence
property_value: dcterms:description "A pattern of hallucinogen use, leading to impairment or distress, as manifested by one to two of the following, occurring at any time in the same 12-month period: 1) Tolerance, as defined by either the following: a. Need for markedly increased amounts of hallucinogen to achieve intoxication or desired effect. b. Markedly diminished effect with continued use of the same amount of hallucinogen; 2) Withdrawal, as manifested by either of the following: a. The characteristic withdrawal syndrome for hallucinogen. b. The same (or closely related) substance is taken to relieve or avoid withdrawal symptoms; 3) hallucinogen is often taken in larger amounts or over a longer period than was intended; 4) There is persistent desire or unsuccessful efforts to cut down or control hallucinogen use; 5) A great deal of time is spent in activities necessary to obtain hallucinogen, use hallucinogen or recover from its effects; 6) Important social, occupational, or recreational activities are given up or reduced because of hallucinogen use; 7) hallucinogen use is continued despite knowledge of having a persistent or recurrent physical or psychological problem that is likely to have been caused or exacerbated by hallucinogen." xsd:string
property_value: isDefinedBy "DSM_IV" xsd:string

[Term]
id: 000047
name: DSM_IV-defined syndromic hallucinogen dependence
is_a: 000045 ! hallucinogen dependence
property_value: dcterms:description "A maladaptive pattern of hallucinogen use, leading to significant impairment or distress, as manifested by three (or more) of the following, occurring at any time in the same 12-month period: 1) Tolerance, as defined by either the following: a. Need for markedly increased amounts of hallucinogen to achieve intoxication or desired effect. b. Markedly diminished effect with continued use of the same amount of hallucinogen; 2) Withdrawal, as manifested by either of the following: a. The characteristic withdrawal syndrome for hallucinogen. b. The same (or closely related) substance is taken to relieve or avoid withdrawal symptoms; 3) hallucinogen is often taken in larger amounts or over a longer period than was intended; 4) There is persistent desire or unsuccessful efforts to cut down or control hallucinogen use; 5) A great deal of time is spent in activities necessary to obtain hallucinogen, use hallucinogen or recover from its effects; 6) Important social, occupational, or recreational activities are given up or reduced because of hallucinogen use; 7) hallucinogen use is continued despite knowledge of having a persistent or recurrent physical or psychological problem that is likely to have been caused or exacerbated by hallucinogen." xsd:string
property_value: isDefinedBy "DSM_IV" xsd:string

[Term]
id: 000048
name: DSM_V-defined mild hallucinogen use disorder
is_a: 000041 ! hallucinogen use disorder
property_value: dcterms:description "A problematic pattern of hallucinogen use leading to clinically significant impairment or distress, as manifested by two of the following, occurring within a 12-month period: 1) hallucinogen is often taken in larger amounts or over a longer period than was intended; 2) There is a persistent desire or unsuccessful efforts to cut down or control hallucinogen use; 3) A great deal of time is spent in activities necessary to obtain hallucinogen, use hallucinogen, or recover from its effects; 4) Craving, or a strong desire or urge to use hallucinogen; 5) Recurrent hallucinogen use resulting in a failure to fulfill major role obligations at work, school, or home; 6) Continued hallucinogen use despite having persistent or recurrent social or interpersonal problems caused or exacerbated by the effects of hallucinogen; 7) Important social, occupational, or recreational activities are given up or reduced because of hallucinogen use; 8) Recurrent hallucinogen use in situations in which it is physically hazardous; 9) hallucinogen use is continued despite knowledge of having a persistent or recurrent physical or psychological problem that is likely to have been caused or exacerbated by hallucinogen; 10) Tolerance, as defined by either of the following:a. A need for markedly increased amounts of hallucinogen to achieve intoxication or desired effect b. A markedly diminished effect with continued use of the same amount of hallucinogen; 11) Withdrawal, as manifested by either of the following: a. The characteristic withdrawal syndrome for hallucinogen. b. hallucinogen (or a closely related substance) is taken to relieve or avoid withdrawal symptoms." xsd:string
property_value: isDefinedBy "DSM_V" xsd:string

[Term]
id: 000049
name: DSM_V-defined moderate hallucinogen use disorder
is_a: 000041 ! hallucinogen use disorder
property_value: dcterms:description "A problematic pattern of hallucinogen use leading to clinically significant impairment or distress, as manifested by 4-5 of the following, occurring within a 12-month period: 1) hallucinogen is often taken in larger amounts or over a longer period than was intended; 2) There is a persistent desire or unsuccessful efforts to cut down or control hallucinogen use; 3) A great deal of time is spent in activities necessary to obtain hallucinogen, use hallucinogen, or recover from its effects; 4) Craving, or a strong desire or urge to use hallucinogen; 5) Recurrent hallucinogen use resulting in a failure to fulfill major role obligations at work, school, or home; 6) Continued hallucinogen use despite having persistent or recurrent social or interpersonal problems caused or exacerbated by the effects of hallucinogen; 7) Important social, occupational, or recreational activities are given up or reduced because of hallucinogen use; 8) Recurrent hallucinogen use in situations in which it is physically hazardous; 9) hallucinogen use is continued despite knowledge of having a persistent or recurrent physical or psychological problem that is likely to have been caused or exacerbated by hallucinogen; 10) Tolerance, as defined by either of the following:a. A need for markedly increased amounts of hallucinogen to achieve intoxication or desired effect b. A markedly diminished effect with continued use of the same amount of hallucinogen; 11) Withdrawal, as manifested by either of the following: a. The characteristic withdrawal syndrome for hallucinogen. b. hallucinogen (or a closely related substance) is taken to relieve or avoid withdrawal symptoms." xsd:string
property_value: isDefinedBy "DSM_V" xsd:string

[Term]
id: 000050
name: DSM_V-defined severe hallucinogen use disorder
is_a: 000041 ! hallucinogen use disorder
property_value: dcterms:description "A problematic pattern of hallucinogen use leading to clinically significant impairment or distress, as manifested by six or more of the following, occurring within a 12-month period: 1) hallucinogen is often taken in larger amounts or over a longer period than was intended; 2) There is a persistent desire or unsuccessful efforts to cut down or control hallucinogen use; 3) A great deal of time is spent in activities necessary to obtain hallucinogen, use hallucinogen, or recover from its effects; 4) Craving, or a strong desire or urge to use hallucinogen; 5) Recurrent hallucinogen use resulting in a failure to fulfill major role obligations at work, school, or home; 6) Continued hallucinogen use despite having persistent or recurrent social or interpersonal problems caused or exacerbated by the effects of hallucinogen; 7) Important social, occupational, or recreational activities are given up or reduced because of hallucinogen use; 8) Recurrent hallucinogen use in situations in which it is physically hazardous; 9) hallucinogen use is continued despite knowledge of having a persistent or recurrent physical or psychological problem that is likely to have been caused or exacerbated by hallucinogen; 10) Tolerance, as defined by either of the following:a. A need for markedly increased amounts of hallucinogen to achieve intoxication or desired effect b. A markedly diminished effect with continued use of the same amount of hallucinogen; 11) Withdrawal, as manifested by either of the following: a. The characteristic withdrawal syndrome for hallucinogen. b. hallucinogen (or a closely related substance) is taken to relieve or avoid withdrawal symptoms." xsd:string
property_value: isDefinedBy "DSM_V" xsd:string

[Term]
id: 000051
name: nicotine use
is_a: 000002 ! substance use
property_value: dcterms:description "A substance use phenotype in which nicotine is used. Use may be through inhalation, injection, ingestion or other means by which the substance may enter the body." xsd:string

[Term]
id: 000052
name: non-repetitive binge nicotine use
is_a: 000006 ! non-repetitive binge substance use
is_a: 000051 ! nicotine use
property_value: dcterms:description "A type of nicotine use characterized by isolated or sporadic use of significant quantities of nicotine in a short time period." xsd:string

[Term]
id: 000053
name: recreational nicotine use
is_a: 000007 ! recreational substance use
is_a: 000051 ! nicotine use
property_value: dcterms:description "A type of nicotine use characterized by occasional limited use of nicotine, without adverse consequences or behavioral/physiologic symptoms of a substance use disorder." xsd:string

[Term]
id: 000054
name: chronic nicotine use
is_a: 000008 ! chronic substance use
is_a: 000051 ! nicotine use
property_value: dcterms:description "A type of nicotine use in which the use of nicotine is frequent and persistent for a period of 3 months or greater; may or may not be accompanied by behavioral or physiologic symptoms necessary to define a substance use disorder." xsd:string

[Term]
id: 000055
name: nicotine use disorder
is_a: 000054 ! chronic nicotine use
property_value: dcterms:description "A type of chronic nicotine use where there is continued use of nicotine despite harm or adverse consequence to self or others. This is defined by behavioral criteria and physiologic symptoms." xsd:string

[Term]
id: 000056
name: nicotine abuse
is_a: 000055 ! nicotine use disorder
property_value: dcterms:description "A type of nicotine use in which the amounts or methods of use of nicotine are harmful or problematic to the individual or others (also called nicotine misuse)" xsd:string

[Term]
id: 000057
name: DSM_IV-defined subsyndromic nicotine abuse
is_a: 000056 ! nicotine abuse
property_value: isDefinedBy "DSM_IV" xsd:string

[Term]
id: 000058
name: DSM_IV-defined syndromic nicotine abuse
is_a: 000056 ! nicotine abuse
property_value: dcterms:description "A maladaptive pattern of nicotine use leading to clinically significant impairment or distress, as manifested by one (or more) of the following, occurring within a 12-month period: 1) Recurrent nicotine use resulting in a failure to fulfill major role obligation at work, school, or home; 2) Recurrent nicotine use in situations in which it is physically hazardous; 3) Recurrent nicotine-related legal problems; 4) Continued nicotine use despite having persistent or recurrent social or interpersonal problems caused or exacerbated by the effects of nicotine." xsd:string
property_value: isDefinedBy "DSM_IV" xsd:string

[Term]
id: 000059
name: nicotine dependence
is_a: 000055 ! nicotine use disorder
property_value: dcterms:description "A type of nicotine use in which the use of nicotine is compulsive and repetitive and may result in tolerance to the effect of the drug and withdrawal symptoms when use is reduced or stopped." xsd:string

[Term]
id: 000060
name: DSM_IV-defined subsyndromic nicotine dependence
is_a: 000059 ! nicotine dependence
property_value: dcterms:description "A pattern of nicotine use, leading to impairment or distress, as manifested by one to two of the following, occurring at any time in the same 12-month period: 1) Tolerance, as defined by either the following: a. Need for markedly increased amounts of nicotine to achieve intoxication or desired effect. b. Markedly diminished effect with continued use of the same amount of nicotine; 2) Withdrawal, as manifested by either of the following: a. The characteristic withdrawal syndrome for nicotine. b. The same (or closely related) substance is taken to relieve or avoid withdrawal symptoms; 3) nicotine is often taken in larger amounts or over a longer period than was intended; 4) There is persistent desire or unsuccessful efforts to cut down or control nicotine use; 5) A great deal of time is spent in activities necessary to obtain nicotine, use nicotine or recover from its effects; 6) Important social, occupational, or recreational activities are given up or reduced because of nicotine use; 7) nicotine use is continued despite knowledge of having a persistent or recurrent physical or psychological problem that is likely to have been caused or exacerbated by nicotine." xsd:string
property_value: isDefinedBy "DSM_IV" xsd:string

[Term]
id: 000061
name: DSM_IV-defined syndromic nicotine dependence
is_a: 000059 ! nicotine dependence
property_value: dcterms:description "A maladaptive pattern of nicotine use, leading to significant impairment or distress, as manifested by three (or more) of the following, occurring at any time in the same 12-month period: 1) Tolerance, as defined by either the following: a. Need for markedly increased amounts of nicotine to achieve intoxication or desired effect. b. Markedly diminished effect with continued use of the same amount of nicotine; 2) Withdrawal, as manifested by either of the following: a. The characteristic withdrawal syndrome for nicotine. b. The same (or closely related) substance is taken to relieve or avoid withdrawal symptoms; 3) nicotine is often taken in larger amounts or over a longer period than was intended; 4) There is persistent desire or unsuccessful efforts to cut down or control nicotine use; 5) A great deal of time is spent in activities necessary to obtain nicotine, use nicotine or recover from its effects; 6) Important social, occupational, or recreational activities are given up or reduced because of nicotine use; 7) nicotine use is continued despite knowledge of having a persistent or recurrent physical or psychological problem that is likely to have been caused or exacerbated by nicotine." xsd:string
property_value: isDefinedBy "DSM_IV" xsd:string

[Term]
id: 000062
name: DSM_V-defined mild nicotine use disorder
is_a: 000055 ! nicotine use disorder
property_value: dcterms:description "A problematic pattern of nicotine use leading to clinically significant impairment or distress, as manifested by two of the following, occurring within a 12-month period: 1) nicotine is often taken in larger amounts or over a longer period than was intended; 2) There is a persistent desire or unsuccessful efforts to cut down or control nicotine use; 3) A great deal of time is spent in activities necessary to obtain nicotine, use nicotine, or recover from its effects; 4) Craving, or a strong desire or urge to use nicotine; 5) Recurrent nicotine use resulting in a failure to fulfill major role obligations at work, school, or home; 6) Continued nicotine use despite having persistent or recurrent social or interpersonal problems caused or exacerbated by the effects of nicotine; 7) Important social, occupational, or recreational activities are given up or reduced because of nicotine use; 8) Recurrent nicotine use in situations in which it is physically hazardous; 9) nicotine use is continued despite knowledge of having a persistent or recurrent physical or psychological problem that is likely to have been caused or exacerbated by nicotine; 10) Tolerance, as defined by either of the following:a. A need for markedly increased amounts of nicotine to achieve intoxication or desired effect b. A markedly diminished effect with continued use of the same amount of nicotine; 11) Withdrawal, as manifested by either of the following: a. The characteristic withdrawal syndrome for nicotine. b. nicotine (or a closely related substance) is taken to relieve or avoid withdrawal symptoms." xsd:string
property_value: isDefinedBy "DSM_V" xsd:string

[Term]
id: 000063
name: DSM_V-defined moderate nicotine use disorder
is_a: 000055 ! nicotine use disorder
property_value: dcterms:description "A problematic pattern of nicotine use leading to clinically significant impairment or distress, as manifested by 4-5 of the following, occurring within a 12-month period: 1) nicotine is often taken in larger amounts or over a longer period than was intended; 2) There is a persistent desire or unsuccessful efforts to cut down or control nicotine use; 3) A great deal of time is spent in activities necessary to obtain nicotine, use nicotine, or recover from its effects; 4) Craving, or a strong desire or urge to use nicotine; 5) Recurrent nicotine use resulting in a failure to fulfill major role obligations at work, school, or home; 6) Continued nicotine use despite having persistent or recurrent social or interpersonal problems caused or exacerbated by the effects of nicotine; 7) Important social, occupational, or recreational activities are given up or reduced because of nicotine use; 8) Recurrent nicotine use in situations in which it is physically hazardous; 9) nicotine use is continued despite knowledge of having a persistent or recurrent physical or psychological problem that is likely to have been caused or exacerbated by nicotine; 10) Tolerance, as defined by either of the following:a. A need for markedly increased amounts of nicotine to achieve intoxication or desired effect b. A markedly diminished effect with continued use of the same amount of nicotine; 11) Withdrawal, as manifested by either of the following: a. The characteristic withdrawal syndrome for nicotine. b. nicotine (or a closely related substance) is taken to relieve or avoid withdrawal symptoms." xsd:string
property_value: isDefinedBy "DSM_V" xsd:string

[Term]
id: 000064
name: DSM_V-defined severe nicotine use disorder
is_a: 000055 ! nicotine use disorder
property_value: dcterms:description "A problematic pattern of nicotine use leading to clinically significant impairment or distress, as manifested by six or more of the following, occurring within a 12-month period: 1) nicotine is often taken in larger amounts or over a longer period than was intended; 2) There is a persistent desire or unsuccessful efforts to cut down or control nicotine use; 3) A great deal of time is spent in activities necessary to obtain nicotine, use nicotine, or recover from its effects; 4) Craving, or a strong desire or urge to use nicotine; 5) Recurrent nicotine use resulting in a failure to fulfill major role obligations at work, school, or home; 6) Continued nicotine use despite having persistent or recurrent social or interpersonal problems caused or exacerbated by the effects of nicotine; 7) Important social, occupational, or recreational activities are given up or reduced because of nicotine use; 8) Recurrent nicotine use in situations in which it is physically hazardous; 9) nicotine use is continued despite knowledge of having a persistent or recurrent physical or psychological problem that is likely to have been caused or exacerbated by nicotine; 10) Tolerance, as defined by either of the following:a. A need for markedly increased amounts of nicotine to achieve intoxication or desired effect b. A markedly diminished effect with continued use of the same amount of nicotine; 11) Withdrawal, as manifested by either of the following: a. The characteristic withdrawal syndrome for nicotine. b. nicotine (or a closely related substance) is taken to relieve or avoid withdrawal symptoms." xsd:string
property_value: isDefinedBy "DSM_V" xsd:string

[Term]
id: 000065
name: opioid use
is_a: 000002 ! substance use
property_value: dcterms:description "A substance use phenotype in which opioid is used. Use may be through inhalation, injection, ingestion or other means by which the substance may enter the body." xsd:string

[Term]
id: 000066
name: non-repetitive binge opioid use
is_a: 000006 ! non-repetitive binge substance use
is_a: 000065 ! opioid use
property_value: dcterms:description "A type of opioid use characterized by isolated or sporadic use of significant quantities of opioid in a short time period." xsd:string

[Term]
id: 000067
name: recreational opioid use
is_a: 000007 ! recreational substance use
is_a: 000065 ! opioid use
property_value: dcterms:description "A type of opioid use characterized by occasional limited use of opioid, without adverse consequences or behavioral/physiologic symptoms of a substance use disorder." xsd:string

[Term]
id: 000068
name: chronic opioid use
is_a: 000008 ! chronic substance use
is_a: 000065 ! opioid use
property_value: dcterms:description "A type of opioid use in which the use of opioid is frequent and persistent for a period of 3 months or greater; may or may not be accompanied by behavioral or physiologic symptoms necessary to define a substance use disorder." xsd:string

[Term]
id: 000069
name: opioid use disorder
is_a: 000068 ! chronic opioid use
property_value: dcterms:description "A type of chronic opioid use where there is continued use of opioid despite harm or adverse consequence to self or others. This is defined by behavioral criteria and physiologic symptoms." xsd:string

[Term]
id: 000070
name: opioid abuse
is_a: 000069 ! opioid use disorder
property_value: dcterms:description "A type of opioid use in which the amounts or methods of use of opioid are harmful or problematic to the individual or others (also called opioid misuse)" xsd:string

[Term]
id: 000071
name: DSM_IV-defined subsyndromic opioid abuse
is_a: 000070 ! opioid abuse
property_value: isDefinedBy "DSM_IV" xsd:string

[Term]
id: 000072
name: DSM_IV-defined syndromic opioid abuse
is_a: 000070 ! opioid abuse
property_value: dcterms:description "A maladaptive pattern of opioid use leading to clinically significant impairment or distress, as manifested by one (or more) of the following, occurring within a 12-month period: 1) Recurrent opioid use resulting in a failure to fulfill major role obligation at work, school, or home; 2) Recurrent opioid use in situations in which it is physically hazardous; 3) Recurrent opioid-related legal problems; 4) Continued opioid use despite having persistent or recurrent social or interpersonal problems caused or exacerbated by the effects of opioid." xsd:string
property_value: isDefinedBy "DSM_IV" xsd:string

[Term]
id: 000073
name: opioid dependence
is_a: 000069 ! opioid use disorder
property_value: dcterms:description "A type of opioid use in which the use of opioid is compulsive and repetitive and may result in tolerance to the effect of the drug and withdrawal symptoms when use is reduced or stopped." xsd:string

[Term]
id: 000074
name: DSM_IV-defined subsyndromic opioid dependence
is_a: 000073 ! opioid dependence
property_value: dcterms:description "A pattern of opioid use, leading to impairment or distress, as manifested by one to two of the following, occurring at any time in the same 12-month period: 1) Tolerance, as defined by either the following: a. Need for markedly increased amounts of opioid to achieve intoxication or desired effect. b. Markedly diminished effect with continued use of the same amount of opioid; 2) Withdrawal, as manifested by either of the following: a. The characteristic withdrawal syndrome for opioid. b. The same (or closely related) substance is taken to relieve or avoid withdrawal symptoms; 3) opioid is often taken in larger amounts or over a longer period than was intended; 4) There is persistent desire or unsuccessful efforts to cut down or control opioid use; 5) A great deal of time is spent in activities necessary to obtain opioid, use opioid or recover from its effects; 6) Important social, occupational, or recreational activities are given up or reduced because of opioid use; 7) opioid use is continued despite knowledge of having a persistent or recurrent physical or psychological problem that is likely to have been caused or exacerbated by opioid." xsd:string
property_value: isDefinedBy "DSM_IV" xsd:string

[Term]
id: 000075
name: DSM_IV-defined syndromic opioid dependence
is_a: 000073 ! opioid dependence
property_value: dcterms:description "A maladaptive pattern of opioid use, leading to significant impairment or distress, as manifested by three (or more) of the following, occurring at any time in the same 12-month period: 1) Tolerance, as defined by either the following: a. Need for markedly increased amounts of opioid to achieve intoxication or desired effect. b. Markedly diminished effect with continued use of the same amount of opioid; 2) Withdrawal, as manifested by either of the following: a. The characteristic withdrawal syndrome for opioid. b. The same (or closely related) substance is taken to relieve or avoid withdrawal symptoms; 3) opioid is often taken in larger amounts or over a longer period than was intended; 4) There is persistent desire or unsuccessful efforts to cut down or control opioid use; 5) A great deal of time is spent in activities necessary to obtain opioid, use opioid or recover from its effects; 6) Important social, occupational, or recreational activities are given up or reduced because of opioid use; 7) opioid use is continued despite knowledge of having a persistent or recurrent physical or psychological problem that is likely to have been caused or exacerbated by opioid." xsd:string
property_value: isDefinedBy "DSM_IV" xsd:string

[Term]
id: 000076
name: DSM_V-defined mild opioid use disorder
is_a: 000069 ! opioid use disorder
property_value: dcterms:description "A problematic pattern of opioid use leading to clinically significant impairment or distress, as manifested by two of the following, occurring within a 12-month period: 1) opioid is often taken in larger amounts or over a longer period than was intended; 2) There is a persistent desire or unsuccessful efforts to cut down or control opioid use; 3) A great deal of time is spent in activities necessary to obtain opioid, use opioid, or recover from its effects; 4) Craving, or a strong desire or urge to use opioid; 5) Recurrent opioid use resulting in a failure to fulfill major role obligations at work, school, or home; 6) Continued opioid use despite having persistent or recurrent social or interpersonal problems caused or exacerbated by the effects of opioid; 7) Important social, occupational, or recreational activities are given up or reduced because of opioid use; 8) Recurrent opioid use in situations in which it is physically hazardous; 9) opioid use is continued despite knowledge of having a persistent or recurrent physical or psychological problem that is likely to have been caused or exacerbated by opioid; 10) Tolerance, as defined by either of the following:a. A need for markedly increased amounts of opioid to achieve intoxication or desired effect b. A markedly diminished effect with continued use of the same amount of opioid; 11) Withdrawal, as manifested by either of the following: a. The characteristic withdrawal syndrome for opioid. b. opioid (or a closely related substance) is taken to relieve or avoid withdrawal symptoms." xsd:string
property_value: isDefinedBy "DSM_V" xsd:string

[Term]
id: 000077
name: DSM_V-defined moderate opioid use disorder
is_a: 000069 ! opioid use disorder
property_value: dcterms:description "A problematic pattern of opioid use leading to clinically significant impairment or distress, as manifested by 4-5 of the following, occurring within a 12-month period: 1) opioid is often taken in larger amounts or over a longer period than was intended; 2) There is a persistent desire or unsuccessful efforts to cut down or control opioid use; 3) A great deal of time is spent in activities necessary to obtain opioid, use opioid, or recover from its effects; 4) Craving, or a strong desire or urge to use opioid; 5) Recurrent opioid use resulting in a failure to fulfill major role obligations at work, school, or home; 6) Continued opioid use despite having persistent or recurrent social or interpersonal problems caused or exacerbated by the effects of opioid; 7) Important social, occupational, or recreational activities are given up or reduced because of opioid use; 8) Recurrent opioid use in situations in which it is physically hazardous; 9) opioid use is continued despite knowledge of having a persistent or recurrent physical or psychological problem that is likely to have been caused or exacerbated by opioid; 10) Tolerance, as defined by either of the following:a. A need for markedly increased amounts of opioid to achieve intoxication or desired effect b. A markedly diminished effect with continued use of the same amount of opioid; 11) Withdrawal, as manifested by either of the following: a. The characteristic withdrawal syndrome for opioid. b. opioid (or a closely related substance) is taken to relieve or avoid withdrawal symptoms." xsd:string
property_value: isDefinedBy "DSM_V" xsd:string

[Term]
id: 000078
name: DSM_V-defined severe opioid use disorder
is_a: 000069 ! opioid use disorder
property_value: dcterms:description "A problematic pattern of opioid use leading to clinically significant impairment or distress, as manifested by six or more of the following, occurring within a 12-month period: 1) opioid is often taken in larger amounts or over a longer period than was intended; 2) There is a persistent desire or unsuccessful efforts to cut down or control opioid use; 3) A great deal of time is spent in activities necessary to obtain opioid, use opioid, or recover from its effects; 4) Craving, or a strong desire or urge to use opioid; 5) Recurrent opioid use resulting in a failure to fulfill major role obligations at work, school, or home; 6) Continued opioid use despite having persistent or recurrent social or interpersonal problems caused or exacerbated by the effects of opioid; 7) Important social, occupational, or recreational activities are given up or reduced because of opioid use; 8) Recurrent opioid use in situations in which it is physically hazardous; 9) opioid use is continued despite knowledge of having a persistent or recurrent physical or psychological problem that is likely to have been caused or exacerbated by opioid; 10) Tolerance, as defined by either of the following:a. A need for markedly increased amounts of opioid to achieve intoxication or desired effect b. A markedly diminished effect with continued use of the same amount of opioid; 11) Withdrawal, as manifested by either of the following: a. The characteristic withdrawal syndrome for opioid. b. opioid (or a closely related substance) is taken to relieve or avoid withdrawal symptoms." xsd:string
property_value: isDefinedBy "DSM_V" xsd:string

[Term]
id: 000079
name: polysubstance use
is_a: 000002 ! substance use
property_value: dcterms:description "A substance use phenotype in which polysubstance is used. Use may be through inhalation, injection, ingestion or other means by which the substance may enter the body." xsd:string

[Term]
id: 000080
name: non-repetitive binge polysubstance use
is_a: 000006 ! non-repetitive binge substance use
is_a: 000079 ! polysubstance use
property_value: dcterms:description "A type of polysubstance use characterized by isolated or sporadic use of significant quantities of polysubstance in a short time period." xsd:string

[Term]
id: 000081
name: recreational polysubstance use
is_a: 000007 ! recreational substance use
is_a: 000079 ! polysubstance use
property_value: dcterms:description "A type of polysubstance use characterized by occasional limited use of polysubstance, without adverse consequences or behavioral/physiologic symptoms of a substance use disorder." xsd:string

[Term]
id: 000082
name: chronic polysubstance use
is_a: 000008 ! chronic substance use
is_a: 000079 ! polysubstance use
property_value: dcterms:description "A type of polysubstance use in which the use of polysubstance is frequent and persistent for a period of 3 months or greater; may or may not be accompanied by behavioral or physiologic symptoms necessary to define a substance use disorder." xsd:string

[Term]
id: 000083
name: polysubstance use disorder
is_a: 000082 ! chronic polysubstance use
property_value: dcterms:description "A type of chronic polysubstance use where there is continued use of polysubstance despite harm or adverse consequence to self or others. This is defined by behavioral criteria and physiologic symptoms." xsd:string

[Term]
id: 000084
name: polysubstance abuse
is_a: 000083 ! polysubstance use disorder
property_value: dcterms:description "A type of polysubstance use in which the amounts or methods of use of polysubstance are harmful or problematic to the individual or others (also called polysubstance misuse)" xsd:string

[Term]
id: 000085
name: DSM_IV-defined subsyndromic polysubstance abuse
is_a: 000084 ! polysubstance abuse
property_value: isDefinedBy "DSM_IV" xsd:string

[Term]
id: 000086
name: DSM_IV-defined syndromic polysubstance abuse
is_a: 000084 ! polysubstance abuse
property_value: dcterms:description "A maladaptive pattern of polysubstance use leading to clinically significant impairment or distress, as manifested by one (or more) of the following, occurring within a 12-month period: 1) Recurrent polysubstance use resulting in a failure to fulfill major role obligation at work, school, or home; 2) Recurrent polysubstance use in situations in which it is physically hazardous; 3) Recurrent polysubstance-related legal problems; 4) Continued polysubstance use despite having persistent or recurrent social or interpersonal problems caused or exacerbated by the effects of polysubstance." xsd:string
property_value: isDefinedBy "DSM_IV" xsd:string

[Term]
id: 000087
name: polysubstance dependence
is_a: 000083 ! polysubstance use disorder
property_value: dcterms:description "A type of polysubstance use in which the use of polysubstance is compulsive and repetitive and may result in tolerance to the effect of the drug and withdrawal symptoms when use is reduced or stopped." xsd:string

[Term]
id: 000088
name: DSM_IV-defined subsyndromic polysubstance dependence
is_a: 000087 ! polysubstance dependence
property_value: dcterms:description "A pattern of polysubstance use, leading to impairment or distress, as manifested by one to two of the following, occurring at any time in the same 12-month period: 1) Tolerance, as defined by either the following: a. Need for markedly increased amounts of polysubstance to achieve intoxication or desired effect. b. Markedly diminished effect with continued use of the same amount of polysubstance; 2) Withdrawal, as manifested by either of the following: a. The characteristic withdrawal syndrome for polysubstance. b. The same (or closely related) substance is taken to relieve or avoid withdrawal symptoms; 3) polysubstance is often taken in larger amounts or over a longer period than was intended; 4) There is persistent desire or unsuccessful efforts to cut down or control polysubstance use; 5) A great deal of time is spent in activities necessary to obtain polysubstance, use polysubstance or recover from its effects; 6) Important social, occupational, or recreational activities are given up or reduced because of polysubstance use; 7) polysubstance use is continued despite knowledge of having a persistent or recurrent physical or psychological problem that is likely to have been caused or exacerbated by polysubstance." xsd:string
property_value: isDefinedBy "DSM_IV" xsd:string

[Term]
id: 000089
name: DSM_IV-defined syndromic polysubstance dependence
is_a: 000087 ! polysubstance dependence
property_value: dcterms:description "A maladaptive pattern of polysubstance use, leading to significant impairment or distress, as manifested by three (or more) of the following, occurring at any time in the same 12-month period: 1) Tolerance, as defined by either the following: a. Need for markedly increased amounts of polysubstance to achieve intoxication or desired effect. b. Markedly diminished effect with continued use of the same amount of polysubstance; 2) Withdrawal, as manifested by either of the following: a. The characteristic withdrawal syndrome for polysubstance. b. The same (or closely related) substance is taken to relieve or avoid withdrawal symptoms; 3) polysubstance is often taken in larger amounts or over a longer period than was intended; 4) There is persistent desire or unsuccessful efforts to cut down or control polysubstance use; 5) A great deal of time is spent in activities necessary to obtain polysubstance, use polysubstance or recover from its effects; 6) Important social, occupational, or recreational activities are given up or reduced because of polysubstance use; 7) polysubstance use is continued despite knowledge of having a persistent or recurrent physical or psychological problem that is likely to have been caused or exacerbated by polysubstance." xsd:string
property_value: isDefinedBy "DSM_IV" xsd:string

[Term]
id: 000090
name: DSM_V-defined mild polysubstance use disorder
is_a: 000083 ! polysubstance use disorder
property_value: dcterms:description "A problematic pattern of polysubstance use leading to clinically significant impairment or distress, as manifested by two of the following, occurring within a 12-month period: 1) polysubstance is often taken in larger amounts or over a longer period than was intended; 2) There is a persistent desire or unsuccessful efforts to cut down or control polysubstance use; 3) A great deal of time is spent in activities necessary to obtain polysubstance, use polysubstance, or recover from its effects; 4) Craving, or a strong desire or urge to use polysubstance; 5) Recurrent polysubstance use resulting in a failure to fulfill major role obligations at work, school, or home; 6) Continued polysubstance use despite having persistent or recurrent social or interpersonal problems caused or exacerbated by the effects of polysubstance; 7) Important social, occupational, or recreational activities are given up or reduced because of polysubstance use; 8) Recurrent polysubstance use in situations in which it is physically hazardous; 9) polysubstance use is continued despite knowledge of having a persistent or recurrent physical or psychological problem that is likely to have been caused or exacerbated by polysubstance; 10) Tolerance, as defined by either of the following:a. A need for markedly increased amounts of polysubstance to achieve intoxication or desired effect b. A markedly diminished effect with continued use of the same amount of polysubstance; 11) Withdrawal, as manifested by either of the following: a. The characteristic withdrawal syndrome for polysubstance. b. polysubstance (or a closely related substance) is taken to relieve or avoid withdrawal symptoms." xsd:string
property_value: isDefinedBy "DSM_V" xsd:string

[Term]
id: 000091
name: DSM_V-defined moderate polysubstance use disorder
is_a: 000083 ! polysubstance use disorder
property_value: dcterms:description "A problematic pattern of polysubstance use leading to clinically significant impairment or distress, as manifested by 4-5 of the following, occurring within a 12-month period: 1) polysubstance is often taken in larger amounts or over a longer period than was intended; 2) There is a persistent desire or unsuccessful efforts to cut down or control polysubstance use; 3) A great deal of time is spent in activities necessary to obtain polysubstance, use polysubstance, or recover from its effects; 4) Craving, or a strong desire or urge to use polysubstance; 5) Recurrent polysubstance use resulting in a failure to fulfill major role obligations at work, school, or home; 6) Continued polysubstance use despite having persistent or recurrent social or interpersonal problems caused or exacerbated by the effects of polysubstance; 7) Important social, occupational, or recreational activities are given up or reduced because of polysubstance use; 8) Recurrent polysubstance use in situations in which it is physically hazardous; 9) polysubstance use is continued despite knowledge of having a persistent or recurrent physical or psychological problem that is likely to have been caused or exacerbated by polysubstance; 10) Tolerance, as defined by either of the following:a. A need for markedly increased amounts of polysubstance to achieve intoxication or desired effect b. A markedly diminished effect with continued use of the same amount of polysubstance; 11) Withdrawal, as manifested by either of the following: a. The characteristic withdrawal syndrome for polysubstance. b. polysubstance (or a closely related substance) is taken to relieve or avoid withdrawal symptoms." xsd:string
property_value: isDefinedBy "DSM_V" xsd:string

[Term]
id: 000092
name: DSM_V-defined severe polysubstance use disorder
is_a: 000083 ! polysubstance use disorder
property_value: dcterms:description "A problematic pattern of polysubstance use leading to clinically significant impairment or distress, as manifested by six or more of the following, occurring within a 12-month period: 1) polysubstance is often taken in larger amounts or over a longer period than was intended; 2) There is a persistent desire or unsuccessful efforts to cut down or control polysubstance use; 3) A great deal of time is spent in activities necessary to obtain polysubstance, use polysubstance, or recover from its effects; 4) Craving, or a strong desire or urge to use polysubstance; 5) Recurrent polysubstance use resulting in a failure to fulfill major role obligations at work, school, or home; 6) Continued polysubstance use despite having persistent or recurrent social or interpersonal problems caused or exacerbated by the effects of polysubstance; 7) Important social, occupational, or recreational activities are given up or reduced because of polysubstance use; 8) Recurrent polysubstance use in situations in which it is physically hazardous; 9) polysubstance use is continued despite knowledge of having a persistent or recurrent physical or psychological problem that is likely to have been caused or exacerbated by polysubstance; 10) Tolerance, as defined by either of the following:a. A need for markedly increased amounts of polysubstance to achieve intoxication or desired effect b. A markedly diminished effect with continued use of the same amount of polysubstance; 11) Withdrawal, as manifested by either of the following: a. The characteristic withdrawal syndrome for polysubstance. b. polysubstance (or a closely related substance) is taken to relieve or avoid withdrawal symptoms." xsd:string
property_value: isDefinedBy "DSM_V" xsd:string

[Term]
id: 000093
name: sedative use
is_a: 000002 ! substance use
property_value: dcterms:description "A substance use phenotype in which sedative is used. Use may be through inhalation, injection, ingestion or other means by which the substance may enter the body." xsd:string

[Term]
id: 000094
name: non-repetitive binge sedative use
is_a: 000006 ! non-repetitive binge substance use
is_a: 000093 ! sedative use
property_value: dcterms:description "A type of sedative use characterized by isolated or sporadic use of significant quantities of sedative in a short time period." xsd:string

[Term]
id: 000095
name: recreational sedative use
is_a: 000007 ! recreational substance use
is_a: 000093 ! sedative use
property_value: dcterms:description "A type of sedative use characterized by occasional limited use of sedative, without adverse consequences or behavioral/physiologic symptoms of a substance use disorder." xsd:string

[Term]
id: 000096
name: chronic sedative use
is_a: 000008 ! chronic substance use
is_a: 000093 ! sedative use
property_value: dcterms:description "A type of sedative use in which the use of sedative is frequent and persistent for a period of 3 months or greater; may or may not be accompanied by behavioral or physiologic symptoms necessary to define a substance use disorder." xsd:string

[Term]
id: 000097
name: sedative use disorder
is_a: 000096 ! chronic sedative use
property_value: dcterms:description "A type of chronic sedative use where there is continued use of sedative despite harm or adverse consequence to self or others. This is defined by behavioral criteria and physiologic symptoms." xsd:string

[Term]
id: 000098
name: sedative abuse
is_a: 000097 ! sedative use disorder
property_value: dcterms:description "A type of sedative use in which the amounts or methods of use of sedative are harmful or problematic to the individual or others (also called sedative misuse)" xsd:string

[Term]
id: 000099
name: DSM_IV-defined subsyndromic sedative abuse
is_a: 000098 ! sedative abuse
property_value: isDefinedBy "DSM_IV" xsd:string

[Term]
id: 000100
name: DSM_IV-defined syndromic sedative abuse
is_a: 000098 ! sedative abuse
property_value: dcterms:description "A maladaptive pattern of sedative use leading to clinically significant impairment or distress, as manifested by one (or more) of the following, occurring within a 12-month period: 1) Recurrent sedative use resulting in a failure to fulfill major role obligation at work, school, or home; 2) Recurrent sedative use in situations in which it is physically hazardous; 3) Recurrent sedative-related legal problems; 4) Continued sedative use despite having persistent or recurrent social or interpersonal problems caused or exacerbated by the effects of sedative." xsd:string
property_value: isDefinedBy "DSM_IV" xsd:string

[Term]
id: 000101
name: sedative dependence
is_a: 000097 ! sedative use disorder
property_value: dcterms:description "A type of sedative use in which the use of sedative is compulsive and repetitive and may result in tolerance to the effect of the drug and withdrawal symptoms when use is reduced or stopped." xsd:string

[Term]
id: 000102
name: DSM_IV-defined subsyndromic sedative dependence
is_a: 000101 ! sedative dependence
property_value: dcterms:description "A pattern of sedative use, leading to impairment or distress, as manifested by one to two of the following, occurring at any time in the same 12-month period: 1) Tolerance, as defined by either the following: a. Need for markedly increased amounts of sedative to achieve intoxication or desired effect. b. Markedly diminished effect with continued use of the same amount of sedative; 2) Withdrawal, as manifested by either of the following: a. The characteristic withdrawal syndrome for sedative. b. The same (or closely related) substance is taken to relieve or avoid withdrawal symptoms; 3) sedative is often taken in larger amounts or over a longer period than was intended; 4) There is persistent desire or unsuccessful efforts to cut down or control sedative use; 5) A great deal of time is spent in activities necessary to obtain sedative, use sedative or recover from its effects; 6) Important social, occupational, or recreational activities are given up or reduced because of sedative use; 7) sedative use is continued despite knowledge of having a persistent or recurrent physical or psychological problem that is likely to have been caused or exacerbated by sedative." xsd:string
property_value: isDefinedBy "DSM_IV" xsd:string

[Term]
id: 000103
name: DSM_IV-defined syndromic sedative dependence
is_a: 000101 ! sedative dependence
property_value: dcterms:description "A maladaptive pattern of sedative use, leading to significant impairment or distress, as manifested by three (or more) of the following, occurring at any time in the same 12-month period: 1) Tolerance, as defined by either the following: a. Need for markedly increased amounts of sedative to achieve intoxication or desired effect. b. Markedly diminished effect with continued use of the same amount of sedative; 2) Withdrawal, as manifested by either of the following: a. The characteristic withdrawal syndrome for sedative. b. The same (or closely related) substance is taken to relieve or avoid withdrawal symptoms; 3) sedative is often taken in larger amounts or over a longer period than was intended; 4) There is persistent desire or unsuccessful efforts to cut down or control sedative use; 5) A great deal of time is spent in activities necessary to obtain sedative, use sedative or recover from its effects; 6) Important social, occupational, or recreational activities are given up or reduced because of sedative use; 7) sedative use is continued despite knowledge of having a persistent or recurrent physical or psychological problem that is likely to have been caused or exacerbated by sedative." xsd:string
property_value: isDefinedBy "DSM_IV" xsd:string

[Term]
id: 000104
name: DSM_V-defined mild sedative use disorder
is_a: 000097 ! sedative use disorder
property_value: dcterms:description "A problematic pattern of sedative use leading to clinically significant impairment or distress, as manifested by two of the following, occurring within a 12-month period: 1) sedative is often taken in larger amounts or over a longer period than was intended; 2) There is a persistent desire or unsuccessful efforts to cut down or control sedative use; 3) A great deal of time is spent in activities necessary to obtain sedative, use sedative, or recover from its effects; 4) Craving, or a strong desire or urge to use sedative; 5) Recurrent sedative use resulting in a failure to fulfill major role obligations at work, school, or home; 6) Continued sedative use despite having persistent or recurrent social or interpersonal problems caused or exacerbated by the effects of sedative; 7) Important social, occupational, or recreational activities are given up or reduced because of sedative use; 8) Recurrent sedative use in situations in which it is physically hazardous; 9) sedative use is continued despite knowledge of having a persistent or recurrent physical or psychological problem that is likely to have been caused or exacerbated by sedative; 10) Tolerance, as defined by either of the following:a. A need for markedly increased amounts of sedative to achieve intoxication or desired effect b. A markedly diminished effect with continued use of the same amount of sedative; 11) Withdrawal, as manifested by either of the following: a. The characteristic withdrawal syndrome for sedative. b. sedative (or a closely related substance) is taken to relieve or avoid withdrawal symptoms." xsd:string
property_value: isDefinedBy "DSM_V" xsd:string

[Term]
id: 000105
name: DSM_V-defined moderate sedative use disorder
is_a: 000097 ! sedative use disorder
property_value: dcterms:description "A problematic pattern of sedative use leading to clinically significant impairment or distress, as manifested by 4-5 of the following, occurring within a 12-month period: 1) sedative is often taken in larger amounts or over a longer period than was intended; 2) There is a persistent desire or unsuccessful efforts to cut down or control sedative use; 3) A great deal of time is spent in activities necessary to obtain sedative, use sedative, or recover from its effects; 4) Craving, or a strong desire or urge to use sedative; 5) Recurrent sedative use resulting in a failure to fulfill major role obligations at work, school, or home; 6) Continued sedative use despite having persistent or recurrent social or interpersonal problems caused or exacerbated by the effects of sedative; 7) Important social, occupational, or recreational activities are given up or reduced because of sedative use; 8) Recurrent sedative use in situations in which it is physically hazardous; 9) sedative use is continued despite knowledge of having a persistent or recurrent physical or psychological problem that is likely to have been caused or exacerbated by sedative; 10) Tolerance, as defined by either of the following:a. A need for markedly increased amounts of sedative to achieve intoxication or desired effect b. A markedly diminished effect with continued use of the same amount of sedative; 11) Withdrawal, as manifested by either of the following: a. The characteristic withdrawal syndrome for sedative. b. sedative (or a closely related substance) is taken to relieve or avoid withdrawal symptoms." xsd:string
property_value: isDefinedBy "DSM_V" xsd:string

[Term]
id: 000106
name: DSM_V-defined severe sedative use disorder
is_a: 000097 ! sedative use disorder
property_value: dcterms:description "A problematic pattern of sedative use leading to clinically significant impairment or distress, as manifested by six or more of the following, occurring within a 12-month period: 1) sedative is often taken in larger amounts or over a longer period than was intended; 2) There is a persistent desire or unsuccessful efforts to cut down or control sedative use; 3) A great deal of time is spent in activities necessary to obtain sedative, use sedative, or recover from its effects; 4) Craving, or a strong desire or urge to use sedative; 5) Recurrent sedative use resulting in a failure to fulfill major role obligations at work, school, or home; 6) Continued sedative use despite having persistent or recurrent social or interpersonal problems caused or exacerbated by the effects of sedative; 7) Important social, occupational, or recreational activities are given up or reduced because of sedative use; 8) Recurrent sedative use in situations in which it is physically hazardous; 9) sedative use is continued despite knowledge of having a persistent or recurrent physical or psychological problem that is likely to have been caused or exacerbated by sedative; 10) Tolerance, as defined by either of the following:a. A need for markedly increased amounts of sedative to achieve intoxication or desired effect b. A markedly diminished effect with continued use of the same amount of sedative; 11) Withdrawal, as manifested by either of the following: a. The characteristic withdrawal syndrome for sedative. b. sedative (or a closely related substance) is taken to relieve or avoid withdrawal symptoms." xsd:string
property_value: isDefinedBy "DSM_V" xsd:string

[Term]
id: 000107
name: stimulant use
is_a: 000002 ! substance use
property_value: dcterms:description "A substance use phenotype in which stimulant is used. Use may be through inhalation, injection, ingestion or other means by which the substance may enter the body." xsd:string

[Term]
id: 000108
name: non-repetitive binge stimulant use
is_a: 000006 ! non-repetitive binge substance use
is_a: 000107 ! stimulant use
property_value: dcterms:description "A type of stimulant use characterized by isolated or sporadic use of significant quantities of stimulant in a short time period." xsd:string

[Term]
id: 000109
name: recreational stimulant use
is_a: 000007 ! recreational substance use
is_a: 000107 ! stimulant use
property_value: dcterms:description "A type of stimulant use characterized by occasional limited use of stimulant, without adverse consequences or behavioral/physiologic symptoms of a substance use disorder." xsd:string

[Term]
id: 000110
name: chronic stimulant use
is_a: 000008 ! chronic substance use
is_a: 000107 ! stimulant use
property_value: dcterms:description "A type of stimulant use in which the use of stimulant is frequent and persistent for a period of 3 months or greater; may or may not be accompanied by behavioral or physiologic symptoms necessary to define a substance use disorder." xsd:string

[Term]
id: 000111
name: stimulant use disorder
is_a: 000110 ! chronic stimulant use
property_value: dcterms:description "A type of chronic stimulant use where there is continued use of stimulant despite harm or adverse consequence to self or others. This is defined by behavioral criteria and physiologic symptoms." xsd:string

[Term]
id: 000112
name: stimulant abuse
is_a: 000111 ! stimulant use disorder
property_value: dcterms:description "A type of stimulant use in which the amounts or methods of use of stimulant are harmful or problematic to the individual or others (also called stimulant misuse)" xsd:string

[Term]
id: 000113
name: DSM_IV-defined subsyndromic stimulant abuse
is_a: 000112 ! stimulant abuse
property_value: isDefinedBy "DSM_IV" xsd:string

[Term]
id: 000114
name: DSM_IV-defined syndromic stimulant abuse
is_a: 000112 ! stimulant abuse
property_value: dcterms:description "A maladaptive pattern of stimulant use leading to clinically significant impairment or distress, as manifested by one (or more) of the following, occurring within a 12-month period: 1) Recurrent stimulant use resulting in a failure to fulfill major role obligation at work, school, or home; 2) Recurrent stimulant use in situations in which it is physically hazardous; 3) Recurrent stimulant-related legal problems; 4) Continued stimulant use despite having persistent or recurrent social or interpersonal problems caused or exacerbated by the effects of stimulant." xsd:string
property_value: isDefinedBy "DSM_IV" xsd:string

[Term]
id: 000115
name: stimulant dependence
is_a: 000111 ! stimulant use disorder
property_value: dcterms:description "A type of stimulant use in which the use of stimulant is compulsive and repetitive and may result in tolerance to the effect of the drug and withdrawal symptoms when use is reduced or stopped." xsd:string

[Term]
id: 000116
name: DSM_IV-defined subsyndromic stimulant dependence
is_a: 000115 ! stimulant dependence
property_value: dcterms:description "A pattern of stimulant use, leading to impairment or distress, as manifested by one to two of the following, occurring at any time in the same 12-month period: 1) Tolerance, as defined by either the following: a. Need for markedly increased amounts of stimulant to achieve intoxication or desired effect. b. Markedly diminished effect with continued use of the same amount of stimulant; 2) Withdrawal, as manifested by either of the following: a. The characteristic withdrawal syndrome for stimulant. b. The same (or closely related) substance is taken to relieve or avoid withdrawal symptoms; 3) stimulant is often taken in larger amounts or over a longer period than was intended; 4) There is persistent desire or unsuccessful efforts to cut down or control stimulant use; 5) A great deal of time is spent in activities necessary to obtain stimulant, use stimulant or recover from its effects; 6) Important social, occupational, or recreational activities are given up or reduced because of stimulant use; 7) stimulant use is continued despite knowledge of having a persistent or recurrent physical or psychological problem that is likely to have been caused or exacerbated by stimulant." xsd:string
property_value: isDefinedBy "DSM_IV" xsd:string

[Term]
id: 000117
name: DSM_IV-defined syndromic stimulant dependence
is_a: 000115 ! stimulant dependence
property_value: dcterms:description "A maladaptive pattern of stimulant use, leading to significant impairment or distress, as manifested by three (or more) of the following, occurring at any time in the same 12-month period: 1) Tolerance, as defined by either the following: a. Need for markedly increased amounts of stimulant to achieve intoxication or desired effect. b. Markedly diminished effect with continued use of the same amount of stimulant; 2) Withdrawal, as manifested by either of the following: a. The characteristic withdrawal syndrome for stimulant. b. The same (or closely related) substance is taken to relieve or avoid withdrawal symptoms; 3) stimulant is often taken in larger amounts or over a longer period than was intended; 4) There is persistent desire or unsuccessful efforts to cut down or control stimulant use; 5) A great deal of time is spent in activities necessary to obtain stimulant, use stimulant or recover from its effects; 6) Important social, occupational, or recreational activities are given up or reduced because of stimulant use; 7) stimulant use is continued despite knowledge of having a persistent or recurrent physical or psychological problem that is likely to have been caused or exacerbated by stimulant." xsd:string
property_value: isDefinedBy "DSM_IV" xsd:string

[Term]
id: 000118
name: DSM_V-defined mild stimulant use disorder
is_a: 000111 ! stimulant use disorder
property_value: dcterms:description "A problematic pattern of stimulant use leading to clinically significant impairment or distress, as manifested by two of the following, occurring within a 12-month period: 1) stimulant is often taken in larger amounts or over a longer period than was intended; 2) There is a persistent desire or unsuccessful efforts to cut down or control stimulant use; 3) A great deal of time is spent in activities necessary to obtain stimulant, use stimulant, or recover from its effects; 4) Craving, or a strong desire or urge to use stimulant; 5) Recurrent stimulant use resulting in a failure to fulfill major role obligations at work, school, or home; 6) Continued stimulant use despite having persistent or recurrent social or interpersonal problems caused or exacerbated by the effects of stimulant; 7) Important social, occupational, or recreational activities are given up or reduced because of stimulant use; 8) Recurrent stimulant use in situations in which it is physically hazardous; 9) stimulant use is continued despite knowledge of having a persistent or recurrent physical or psychological problem that is likely to have been caused or exacerbated by stimulant; 10) Tolerance, as defined by either of the following:a. A need for markedly increased amounts of stimulant to achieve intoxication or desired effect b. A markedly diminished effect with continued use of the same amount of stimulant; 11) Withdrawal, as manifested by either of the following: a. The characteristic withdrawal syndrome for stimulant. b. stimulant (or a closely related substance) is taken to relieve or avoid withdrawal symptoms." xsd:string
property_value: isDefinedBy "DSM_V" xsd:string

[Term]
id: 000119
name: DSM_V-defined moderate stimulant use disorder
is_a: 000111 ! stimulant use disorder
property_value: dcterms:description "A problematic pattern of stimulant use leading to clinically significant impairment or distress, as manifested by 4-5 of the following, occurring within a 12-month period: 1) stimulant is often taken in larger amounts or over a longer period than was intended; 2) There is a persistent desire or unsuccessful efforts to cut down or control stimulant use; 3) A great deal of time is spent in activities necessary to obtain stimulant, use stimulant, or recover from its effects; 4) Craving, or a strong desire or urge to use stimulant; 5) Recurrent stimulant use resulting in a failure to fulfill major role obligations at work, school, or home; 6) Continued stimulant use despite having persistent or recurrent social or interpersonal problems caused or exacerbated by the effects of stimulant; 7) Important social, occupational, or recreational activities are given up or reduced because of stimulant use; 8) Recurrent stimulant use in situations in which it is physically hazardous; 9) stimulant use is continued despite knowledge of having a persistent or recurrent physical or psychological problem that is likely to have been caused or exacerbated by stimulant; 10) Tolerance, as defined by either of the following:a. A need for markedly increased amounts of stimulant to achieve intoxication or desired effect b. A markedly diminished effect with continued use of the same amount of stimulant; 11) Withdrawal, as manifested by either of the following: a. The characteristic withdrawal syndrome for stimulant. b. stimulant (or a closely related substance) is taken to relieve or avoid withdrawal symptoms." xsd:string
property_value: isDefinedBy "DSM_V" xsd:string

[Term]
id: 000120
name: DSM_V-defined severe stimulant use disorder
is_a: 000111 ! stimulant use disorder
property_value: dcterms:description "A problematic pattern of stimulant use leading to clinically significant impairment or distress, as manifested by six or more of the following, occurring within a 12-month period: 1) stimulant is often taken in larger amounts or over a longer period than was intended; 2) There is a persistent desire or unsuccessful efforts to cut down or control stimulant use; 3) A great deal of time is spent in activities necessary to obtain stimulant, use stimulant, or recover from its effects; 4) Craving, or a strong desire or urge to use stimulant; 5) Recurrent stimulant use resulting in a failure to fulfill major role obligations at work, school, or home; 6) Continued stimulant use despite having persistent or recurrent social or interpersonal problems caused or exacerbated by the effects of stimulant; 7) Important social, occupational, or recreational activities are given up or reduced because of stimulant use; 8) Recurrent stimulant use in situations in which it is physically hazardous; 9) stimulant use is continued despite knowledge of having a persistent or recurrent physical or psychological problem that is likely to have been caused or exacerbated by stimulant; 10) Tolerance, as defined by either of the following:a. A need for markedly increased amounts of stimulant to achieve intoxication or desired effect b. A markedly diminished effect with continued use of the same amount of stimulant; 11) Withdrawal, as manifested by either of the following: a. The characteristic withdrawal syndrome for stimulant. b. stimulant (or a closely related substance) is taken to relieve or avoid withdrawal symptoms." xsd:string
property_value: isDefinedBy "DSM_V" xsd:string

[Term]
id: 000121
name: amphetamine use
is_a: 000107 ! stimulant use
property_value: dcterms:description "A substance use phenotype in which amphetamine is used. Use may be through inhalation, injection, ingestion or other means by which the substance may enter the body." xsd:string

[Term]
id: 000122
name: non-repetitive binge amphetamine use
is_a: 000006 ! non-repetitive binge substance use
is_a: 000121 ! amphetamine use
property_value: dcterms:description "A type of amphetamine use characterized by isolated or sporadic use of significant quantities of amphetamine in a short time period." xsd:string

[Term]
id: 000123
name: recreational amphetamine use
is_a: 000007 ! recreational substance use
is_a: 000121 ! amphetamine use
property_value: dcterms:description "A type of amphetamine use characterized by occasional limited use of amphetamine, without adverse consequences or behavioral/physiologic symptoms of a substance use disorder." xsd:string

[Term]
id: 000124
name: chronic amphetamine use
is_a: 000008 ! chronic substance use
is_a: 000121 ! amphetamine use
property_value: dcterms:description "A type of amphetamine use in which the use of amphetamine is frequent and persistent for a period of 3 months or greater; may or may not be accompanied by behavioral or physiologic symptoms necessary to define a substance use disorder." xsd:string

[Term]
id: 000125
name: amphetamine use disorder
is_a: 000124 ! chronic amphetamine use
property_value: dcterms:description "A type of chronic amphetamine use where there is continued use of amphetamine despite harm or adverse consequence to self or others. This is defined by behavioral criteria and physiologic symptoms." xsd:string

[Term]
id: 000126
name: amphetamine abuse
is_a: 000125 ! amphetamine use disorder
property_value: dcterms:description "A type of amphetamine use in which the amounts or methods of use of amphetamine are harmful or problematic to the individual or others (also called amphetamine misuse)" xsd:string

[Term]
id: 000127
name: DSM_IV-defined subsyndromic amphetamine abuse
is_a: 000126 ! amphetamine abuse
property_value: isDefinedBy "DSM_IV" xsd:string

[Term]
id: 000128
name: DSM_IV-defined syndromic amphetamine abuse
is_a: 000126 ! amphetamine abuse
property_value: dcterms:description "A maladaptive pattern of amphetamine use leading to clinically significant impairment or distress, as manifested by one (or more) of the following, occurring within a 12-month period: 1) Recurrent amphetamine use resulting in a failure to fulfill major role obligation at work, school, or home; 2) Recurrent amphetamine use in situations in which it is physically hazardous; 3) Recurrent amphetamine-related legal problems; 4) Continued amphetamine use despite having persistent or recurrent social or interpersonal problems caused or exacerbated by the effects of amphetamine." xsd:string
property_value: isDefinedBy "DSM_IV" xsd:string

[Term]
id: 000129
name: amphetamine dependence
is_a: 000125 ! amphetamine use disorder
property_value: dcterms:description "A type of amphetamine use in which the use of amphetamine is compulsive and repetitive and may result in tolerance to the effect of the drug and withdrawal symptoms when use is reduced or stopped." xsd:string

[Term]
id: 000130
name: DSM_IV-defined subsyndromic amphetamine dependence
is_a: 000129 ! amphetamine dependence
property_value: dcterms:description "A pattern of amphetamine use, leading to impairment or distress, as manifested by one to two of the following, occurring at any time in the same 12-month period: 1) Tolerance, as defined by either the following: a. Need for markedly increased amounts of amphetamine to achieve intoxication or desired effect. b. Markedly diminished effect with continued use of the same amount of amphetamine; 2) Withdrawal, as manifested by either of the following: a. The characteristic withdrawal syndrome for amphetamine. b. The same (or closely related) substance is taken to relieve or avoid withdrawal symptoms; 3) amphetamine is often taken in larger amounts or over a longer period than was intended; 4) There is persistent desire or unsuccessful efforts to cut down or control amphetamine use; 5) A great deal of time is spent in activities necessary to obtain amphetamine, use amphetamine or recover from its effects; 6) Important social, occupational, or recreational activities are given up or reduced because of amphetamine use; 7) amphetamine use is continued despite knowledge of having a persistent or recurrent physical or psychological problem that is likely to have been caused or exacerbated by amphetamine." xsd:string
property_value: isDefinedBy "DSM_IV" xsd:string

[Term]
id: 000131
name: DSM_IV-defined syndromic amphetamine dependence
is_a: 000129 ! amphetamine dependence
property_value: dcterms:description "A maladaptive pattern of amphetamine use, leading to significant impairment or distress, as manifested by three (or more) of the following, occurring at any time in the same 12-month period: 1) Tolerance, as defined by either the following: a. Need for markedly increased amounts of amphetamine to achieve intoxication or desired effect. b. Markedly diminished effect with continued use of the same amount of amphetamine; 2) Withdrawal, as manifested by either of the following: a. The characteristic withdrawal syndrome for amphetamine. b. The same (or closely related) substance is taken to relieve or avoid withdrawal symptoms; 3) amphetamine is often taken in larger amounts or over a longer period than was intended; 4) There is persistent desire or unsuccessful efforts to cut down or control amphetamine use; 5) A great deal of time is spent in activities necessary to obtain amphetamine, use amphetamine or recover from its effects; 6) Important social, occupational, or recreational activities are given up or reduced because of amphetamine use; 7) amphetamine use is continued despite knowledge of having a persistent or recurrent physical or psychological problem that is likely to have been caused or exacerbated by amphetamine." xsd:string
property_value: isDefinedBy "DSM_IV" xsd:string

[Term]
id: 000132
name: DSM_V-defined mild amphetamine use disorder
is_a: 000125 ! amphetamine use disorder
property_value: dcterms:description "A problematic pattern of amphetamine use leading to clinically significant impairment or distress, as manifested by two of the following, occurring within a 12-month period: 1) amphetamine is often taken in larger amounts or over a longer period than was intended; 2) There is a persistent desire or unsuccessful efforts to cut down or control amphetamine use; 3) A great deal of time is spent in activities necessary to obtain amphetamine, use amphetamine, or recover from its effects; 4) Craving, or a strong desire or urge to use amphetamine; 5) Recurrent amphetamine use resulting in a failure to fulfill major role obligations at work, school, or home; 6) Continued amphetamine use despite having persistent or recurrent social or interpersonal problems caused or exacerbated by the effects of amphetamine; 7) Important social, occupational, or recreational activities are given up or reduced because of amphetamine use; 8) Recurrent amphetamine use in situations in which it is physically hazardous; 9) amphetamine use is continued despite knowledge of having a persistent or recurrent physical or psychological problem that is likely to have been caused or exacerbated by amphetamine; 10) Tolerance, as defined by either of the following:a. A need for markedly increased amounts of amphetamine to achieve intoxication or desired effect b. A markedly diminished effect with continued use of the same amount of amphetamine; 11) Withdrawal, as manifested by either of the following: a. The characteristic withdrawal syndrome for amphetamine. b. amphetamine (or a closely related substance) is taken to relieve or avoid withdrawal symptoms." xsd:string
property_value: isDefinedBy "DSM_V" xsd:string

[Term]
id: 000133
name: DSM_V-defined moderate amphetamine use disorder
is_a: 000125 ! amphetamine use disorder
property_value: dcterms:description "A problematic pattern of amphetamine use leading to clinically significant impairment or distress, as manifested by 4-5 of the following, occurring within a 12-month period: 1) amphetamine is often taken in larger amounts or over a longer period than was intended; 2) There is a persistent desire or unsuccessful efforts to cut down or control amphetamine use; 3) A great deal of time is spent in activities necessary to obtain amphetamine, use amphetamine, or recover from its effects; 4) Craving, or a strong desire or urge to use amphetamine; 5) Recurrent amphetamine use resulting in a failure to fulfill major role obligations at work, school, or home; 6) Continued amphetamine use despite having persistent or recurrent social or interpersonal problems caused or exacerbated by the effects of amphetamine; 7) Important social, occupational, or recreational activities are given up or reduced because of amphetamine use; 8) Recurrent amphetamine use in situations in which it is physically hazardous; 9) amphetamine use is continued despite knowledge of having a persistent or recurrent physical or psychological problem that is likely to have been caused or exacerbated by amphetamine; 10) Tolerance, as defined by either of the following:a. A need for markedly increased amounts of amphetamine to achieve intoxication or desired effect b. A markedly diminished effect with continued use of the same amount of amphetamine; 11) Withdrawal, as manifested by either of the following: a. The characteristic withdrawal syndrome for amphetamine. b. amphetamine (or a closely related substance) is taken to relieve or avoid withdrawal symptoms." xsd:string
property_value: isDefinedBy "DSM_V" xsd:string

[Term]
id: 000134
name: DSM_V-defined severe amphetamine use disorder
is_a: 000125 ! amphetamine use disorder
property_value: dcterms:description "A problematic pattern of amphetamine use leading to clinically significant impairment or distress, as manifested by six or more of the following, occurring within a 12-month period: 1) amphetamine is often taken in larger amounts or over a longer period than was intended; 2) There is a persistent desire or unsuccessful efforts to cut down or control amphetamine use; 3) A great deal of time is spent in activities necessary to obtain amphetamine, use amphetamine, or recover from its effects; 4) Craving, or a strong desire or urge to use amphetamine; 5) Recurrent amphetamine use resulting in a failure to fulfill major role obligations at work, school, or home; 6) Continued amphetamine use despite having persistent or recurrent social or interpersonal problems caused or exacerbated by the effects of amphetamine; 7) Important social, occupational, or recreational activities are given up or reduced because of amphetamine use; 8) Recurrent amphetamine use in situations in which it is physically hazardous; 9) amphetamine use is continued despite knowledge of having a persistent or recurrent physical or psychological problem that is likely to have been caused or exacerbated by amphetamine; 10) Tolerance, as defined by either of the following:a. A need for markedly increased amounts of amphetamine to achieve intoxication or desired effect b. A markedly diminished effect with continued use of the same amount of amphetamine; 11) Withdrawal, as manifested by either of the following: a. The characteristic withdrawal syndrome for amphetamine. b. amphetamine (or a closely related substance) is taken to relieve or avoid withdrawal symptoms." xsd:string
property_value: isDefinedBy "DSM_V" xsd:string

[Term]
id: 000135
name: methamphetamine use
is_a: 000107 ! stimulant use
property_value: dcterms:description "A substance use phenotype in which methamphetamine is used. Use may be through inhalation, injection, ingestion or other means by which the substance may enter the body." xsd:string

[Term]
id: 000136
name: non-repetitive binge methamphetamine use
is_a: 000006 ! non-repetitive binge substance use
is_a: 000135 ! methamphetamine use
property_value: dcterms:description "A type of methamphetamine use characterized by isolated or sporadic use of significant quantities of methamphetamine in a short time period." xsd:string

[Term]
id: 000137
name: recreational methamphetamine use
is_a: 000007 ! recreational substance use
is_a: 000135 ! methamphetamine use
property_value: dcterms:description "A type of methamphetamine use characterized by occasional limited use of methamphetamine, without adverse consequences or behavioral/physiologic symptoms of a substance use disorder." xsd:string

[Term]
id: 000138
name: chronic methamphetamine use
is_a: 000008 ! chronic substance use
is_a: 000135 ! methamphetamine use
property_value: dcterms:description "A type of methamphetamine use in which the use of methamphetamine is frequent and persistent for a period of 3 months or greater; may or may not be accompanied by behavioral or physiologic symptoms necessary to define a substance use disorder." xsd:string

[Term]
id: 000139
name: methamphetamine use disorder
is_a: 000138 ! chronic methamphetamine use
property_value: dcterms:description "A type of chronic methamphetamine use where there is continued use of methamphetamine despite harm or adverse consequence to self or others. This is defined by behavioral criteria and physiologic symptoms." xsd:string

[Term]
id: 000140
name: methamphetamine abuse
is_a: 000139 ! methamphetamine use disorder
property_value: dcterms:description "A type of methamphetamine use in which the amounts or methods of use of methamphetamine are harmful or problematic to the individual or others (also called methamphetamine misuse)" xsd:string

[Term]
id: 000141
name: DSM_IV-defined subsyndromic methamphetamine abuse
is_a: 000140 ! methamphetamine abuse
property_value: isDefinedBy "DSM_IV" xsd:string

[Term]
id: 000142
name: DSM_IV-defined syndromic methamphetamine abuse
is_a: 000140 ! methamphetamine abuse
property_value: dcterms:description "A maladaptive pattern of methamphetamine use leading to clinically significant impairment or distress, as manifested by one (or more) of the following, occurring within a 12-month period: 1) Recurrent methamphetamine use resulting in a failure to fulfill major role obligation at work, school, or home; 2) Recurrent methamphetamine use in situations in which it is physically hazardous; 3) Recurrent methamphetamine-related legal problems; 4) Continued methamphetamine use despite having persistent or recurrent social or interpersonal problems caused or exacerbated by the effects of methamphetamine." xsd:string
property_value: isDefinedBy "DSM_IV" xsd:string

[Term]
id: 000143
name: methamphetamine dependence
is_a: 000139 ! methamphetamine use disorder
property_value: dcterms:description "A type of methamphetamine use in which the use of methamphetamine is compulsive and repetitive and may result in tolerance to the effect of the drug and withdrawal symptoms when use is reduced or stopped." xsd:string

[Term]
id: 000144
name: DSM_IV-defined subsyndromic methamphetamine dependence
is_a: 000143 ! methamphetamine dependence
property_value: dcterms:description "A pattern of methamphetamine use, leading to impairment or distress, as manifested by one to two of the following, occurring at any time in the same 12-month period: 1) Tolerance, as defined by either the following: a. Need for markedly increased amounts of methamphetamine to achieve intoxication or desired effect. b. Markedly diminished effect with continued use of the same amount of methamphetamine; 2) Withdrawal, as manifested by either of the following: a. The characteristic withdrawal syndrome for methamphetamine. b. The same (or closely related) substance is taken to relieve or avoid withdrawal symptoms; 3) methamphetamine is often taken in larger amounts or over a longer period than was intended; 4) There is persistent desire or unsuccessful efforts to cut down or control methamphetamine use; 5) A great deal of time is spent in activities necessary to obtain methamphetamine, use methamphetamine or recover from its effects; 6) Important social, occupational, or recreational activities are given up or reduced because of methamphetamine use; 7) methamphetamine use is continued despite knowledge of having a persistent or recurrent physical or psychological problem that is likely to have been caused or exacerbated by methamphetamine." xsd:string
property_value: isDefinedBy "DSM_IV" xsd:string

[Term]
id: 000145
name: DSM_IV-defined syndromic methamphetamine dependence
is_a: 000143 ! methamphetamine dependence
property_value: dcterms:description "A maladaptive pattern of methamphetamine use, leading to significant impairment or distress, as manifested by three (or more) of the following, occurring at any time in the same 12-month period: 1) Tolerance, as defined by either the following: a. Need for markedly increased amounts of methamphetamine to achieve intoxication or desired effect. b. Markedly diminished effect with continued use of the same amount of methamphetamine; 2) Withdrawal, as manifested by either of the following: a. The characteristic withdrawal syndrome for methamphetamine. b. The same (or closely related) substance is taken to relieve or avoid withdrawal symptoms; 3) methamphetamine is often taken in larger amounts or over a longer period than was intended; 4) There is persistent desire or unsuccessful efforts to cut down or control methamphetamine use; 5) A great deal of time is spent in activities necessary to obtain methamphetamine, use methamphetamine or recover from its effects; 6) Important social, occupational, or recreational activities are given up or reduced because of methamphetamine use; 7) methamphetamine use is continued despite knowledge of having a persistent or recurrent physical or psychological problem that is likely to have been caused or exacerbated by methamphetamine." xsd:string
property_value: isDefinedBy "DSM_IV" xsd:string

[Term]
id: 000146
name: DSM_V-defined mild methamphetamine use disorder
is_a: 000139 ! methamphetamine use disorder
property_value: dcterms:description "A problematic pattern of methamphetamine use leading to clinically significant impairment or distress, as manifested by two of the following, occurring within a 12-month period: 1) methamphetamine is often taken in larger amounts or over a longer period than was intended; 2) There is a persistent desire or unsuccessful efforts to cut down or control methamphetamine use; 3) A great deal of time is spent in activities necessary to obtain methamphetamine, use methamphetamine, or recover from its effects; 4) Craving, or a strong desire or urge to use methamphetamine; 5) Recurrent methamphetamine use resulting in a failure to fulfill major role obligations at work, school, or home; 6) Continued methamphetamine use despite having persistent or recurrent social or interpersonal problems caused or exacerbated by the effects of methamphetamine; 7) Important social, occupational, or recreational activities are given up or reduced because of methamphetamine use; 8) Recurrent methamphetamine use in situations in which it is physically hazardous; 9) methamphetamine use is continued despite knowledge of having a persistent or recurrent physical or psychological problem that is likely to have been caused or exacerbated by methamphetamine; 10) Tolerance, as defined by either of the following:a. A need for markedly increased amounts of methamphetamine to achieve intoxication or desired effect b. A markedly diminished effect with continued use of the same amount of methamphetamine; 11) Withdrawal, as manifested by either of the following: a. The characteristic withdrawal syndrome for methamphetamine. b. methamphetamine (or a closely related substance) is taken to relieve or avoid withdrawal symptoms." xsd:string
property_value: isDefinedBy "DSM_V" xsd:string

[Term]
id: 000147
name: DSM_V-defined moderate methamphetamine use disorder
is_a: 000139 ! methamphetamine use disorder
property_value: dcterms:description "A problematic pattern of methamphetamine use leading to clinically significant impairment or distress, as manifested by 4-5 of the following, occurring within a 12-month period: 1) methamphetamine is often taken in larger amounts or over a longer period than was intended; 2) There is a persistent desire or unsuccessful efforts to cut down or control methamphetamine use; 3) A great deal of time is spent in activities necessary to obtain methamphetamine, use methamphetamine, or recover from its effects; 4) Craving, or a strong desire or urge to use methamphetamine; 5) Recurrent methamphetamine use resulting in a failure to fulfill major role obligations at work, school, or home; 6) Continued methamphetamine use despite having persistent or recurrent social or interpersonal problems caused or exacerbated by the effects of methamphetamine; 7) Important social, occupational, or recreational activities are given up or reduced because of methamphetamine use; 8) Recurrent methamphetamine use in situations in which it is physically hazardous; 9) methamphetamine use is continued despite knowledge of having a persistent or recurrent physical or psychological problem that is likely to have been caused or exacerbated by methamphetamine; 10) Tolerance, as defined by either of the following:a. A need for markedly increased amounts of methamphetamine to achieve intoxication or desired effect b. A markedly diminished effect with continued use of the same amount of methamphetamine; 11) Withdrawal, as manifested by either of the following: a. The characteristic withdrawal syndrome for methamphetamine. b. methamphetamine (or a closely related substance) is taken to relieve or avoid withdrawal symptoms." xsd:string
property_value: isDefinedBy "DSM_V" xsd:string

[Term]
id: 000148
name: DSM_V-defined severe methamphetamine use disorder
is_a: 000139 ! methamphetamine use disorder
property_value: dcterms:description "A problematic pattern of methamphetamine use leading to clinically significant impairment or distress, as manifested by six or more of the following, occurring within a 12-month period: 1) methamphetamine is often taken in larger amounts or over a longer period than was intended; 2) There is a persistent desire or unsuccessful efforts to cut down or control methamphetamine use; 3) A great deal of time is spent in activities necessary to obtain methamphetamine, use methamphetamine, or recover from its effects; 4) Craving, or a strong desire or urge to use methamphetamine; 5) Recurrent methamphetamine use resulting in a failure to fulfill major role obligations at work, school, or home; 6) Continued methamphetamine use despite having persistent or recurrent social or interpersonal problems caused or exacerbated by the effects of methamphetamine; 7) Important social, occupational, or recreational activities are given up or reduced because of methamphetamine use; 8) Recurrent methamphetamine use in situations in which it is physically hazardous; 9) methamphetamine use is continued despite knowledge of having a persistent or recurrent physical or psychological problem that is likely to have been caused or exacerbated by methamphetamine; 10) Tolerance, as defined by either of the following:a. A need for markedly increased amounts of methamphetamine to achieve intoxication or desired effect b. A markedly diminished effect with continued use of the same amount of methamphetamine; 11) Withdrawal, as manifested by either of the following: a. The characteristic withdrawal syndrome for methamphetamine. b. methamphetamine (or a closely related substance) is taken to relieve or avoid withdrawal symptoms." xsd:string
property_value: isDefinedBy "DSM_V" xsd:string

[Term]
id: 000149
name: cocaine use
is_a: 000107 ! stimulant use
property_value: dcterms:description "A substance use phenotype in which cocaine is used. Use may be through inhalation, injection, ingestion or other means by which the substance may enter the body." xsd:string

[Term]
id: 000150
name: non-repetitive binge cocaine use
is_a: 000006 ! non-repetitive binge substance use
is_a: 000149 ! cocaine use
property_value: dcterms:description "A type of cocaine use characterized by isolated or sporadic use of significant quantities of cocaine in a short time period." xsd:string

[Term]
id: 000151
name: recreational cocaine use
is_a: 000007 ! recreational substance use
is_a: 000149 ! cocaine use
property_value: dcterms:description "A type of cocaine use characterized by occasional limited use of cocaine, without adverse consequences or behavioral/physiologic symptoms of a substance use disorder." xsd:string

[Term]
id: 000152
name: chronic cocaine use
is_a: 000008 ! chronic substance use
is_a: 000149 ! cocaine use
property_value: dcterms:description "A type of cocaine use in which the use of cocaine is frequent and persistent for a period of 3 months or greater; may or may not be accompanied by behavioral or physiologic symptoms necessary to define a substance use disorder." xsd:string

[Term]
id: 000153
name: cocaine use disorder
is_a: 000152 ! chronic cocaine use
property_value: dcterms:description "A type of chronic cocaine use where there is continued use of cocaine despite harm or adverse consequence to self or others. This is defined by behavioral criteria and physiologic symptoms." xsd:string

[Term]
id: 000154
name: cocaine abuse
is_a: 000153 ! cocaine use disorder
property_value: dcterms:description "A type of cocaine use in which the amounts or methods of use of cocaine are harmful or problematic to the individual or others (also called cocaine misuse)" xsd:string

[Term]
id: 000155
name: DSM_IV-defined subsyndromic cocaine abuse
is_a: 000154 ! cocaine abuse
property_value: isDefinedBy "DSM_IV" xsd:string

[Term]
id: 000156
name: DSM_IV-defined syndromic cocaine abuse
is_a: 000154 ! cocaine abuse
property_value: dcterms:description "A maladaptive pattern of cocaine use leading to clinically significant impairment or distress, as manifested by one (or more) of the following, occurring within a 12-month period: 1) Recurrent cocaine use resulting in a failure to fulfill major role obligation at work, school, or home; 2) Recurrent cocaine use in situations in which it is physically hazardous; 3) Recurrent cocaine-related legal problems; 4) Continued cocaine use despite having persistent or recurrent social or interpersonal problems caused or exacerbated by the effects of cocaine." xsd:string
property_value: isDefinedBy "DSM_IV" xsd:string

[Term]
id: 000157
name: cocaine dependence
is_a: 000153 ! cocaine use disorder
property_value: dcterms:description "A type of cocaine use in which the use of cocaine is compulsive and repetitive and may result in tolerance to the effect of the drug and withdrawal symptoms when use is reduced or stopped." xsd:string

[Term]
id: 000158
name: DSM_IV-defined subsyndromic cocaine dependence
is_a: 000157 ! cocaine dependence
property_value: dcterms:description "A pattern of cocaine use, leading to impairment or distress, as manifested by one to two of the following, occurring at any time in the same 12-month period: 1) Tolerance, as defined by either the following: a. Need for markedly increased amounts of cocaine to achieve intoxication or desired effect. b. Markedly diminished effect with continued use of the same amount of cocaine; 2) Withdrawal, as manifested by either of the following: a. The characteristic withdrawal syndrome for cocaine. b. The same (or closely related) substance is taken to relieve or avoid withdrawal symptoms; 3) cocaine is often taken in larger amounts or over a longer period than was intended; 4) There is persistent desire or unsuccessful efforts to cut down or control cocaine use; 5) A great deal of time is spent in activities necessary to obtain cocaine, use cocaine or recover from its effects; 6) Important social, occupational, or recreational activities are given up or reduced because of cocaine use; 7) cocaine use is continued despite knowledge of having a persistent or recurrent physical or psychological problem that is likely to have been caused or exacerbated by cocaine." xsd:string
property_value: isDefinedBy "DSM_IV" xsd:string

[Term]
id: 000159
name: DSM_IV-defined syndromic cocaine dependence
is_a: 000157 ! cocaine dependence
property_value: dcterms:description "A maladaptive pattern of cocaine use, leading to significant impairment or distress, as manifested by three (or more) of the following, occurring at any time in the same 12-month period: 1) Tolerance, as defined by either the following: a. Need for markedly increased amounts of cocaine to achieve intoxication or desired effect. b. Markedly diminished effect with continued use of the same amount of cocaine; 2) Withdrawal, as manifested by either of the following: a. The characteristic withdrawal syndrome for cocaine. b. The same (or closely related) substance is taken to relieve or avoid withdrawal symptoms; 3) cocaine is often taken in larger amounts or over a longer period than was intended; 4) There is persistent desire or unsuccessful efforts to cut down or control cocaine use; 5) A great deal of time is spent in activities necessary to obtain cocaine, use cocaine or recover from its effects; 6) Important social, occupational, or recreational activities are given up or reduced because of cocaine use; 7) cocaine use is continued despite knowledge of having a persistent or recurrent physical or psychological problem that is likely to have been caused or exacerbated by cocaine." xsd:string
property_value: isDefinedBy "DSM_IV" xsd:string

[Term]
id: 000160
name: DSM_V-defined mild cocaine use disorder
is_a: 000153 ! cocaine use disorder
property_value: dcterms:description "A problematic pattern of cocaine use leading to clinically significant impairment or distress, as manifested by two of the following, occurring within a 12-month period: 1) cocaine is often taken in larger amounts or over a longer period than was intended; 2) There is a persistent desire or unsuccessful efforts to cut down or control cocaine use; 3) A great deal of time is spent in activities necessary to obtain cocaine, use cocaine, or recover from its effects; 4) Craving, or a strong desire or urge to use cocaine; 5) Recurrent cocaine use resulting in a failure to fulfill major role obligations at work, school, or home; 6) Continued cocaine use despite having persistent or recurrent social or interpersonal problems caused or exacerbated by the effects of cocaine; 7) Important social, occupational, or recreational activities are given up or reduced because of cocaine use; 8) Recurrent cocaine use in situations in which it is physically hazardous; 9) cocaine use is continued despite knowledge of having a persistent or recurrent physical or psychological problem that is likely to have been caused or exacerbated by cocaine; 10) Tolerance, as defined by either of the following:a. A need for markedly increased amounts of cocaine to achieve intoxication or desired effect b. A markedly diminished effect with continued use of the same amount of cocaine; 11) Withdrawal, as manifested by either of the following: a. The characteristic withdrawal syndrome for cocaine. b. cocaine (or a closely related substance) is taken to relieve or avoid withdrawal symptoms." xsd:string
property_value: isDefinedBy "DSM_V" xsd:string

[Term]
id: 000161
name: DSM_V-defined moderate cocaine use disorder
is_a: 000153 ! cocaine use disorder
property_value: dcterms:description "A problematic pattern of cocaine use leading to clinically significant impairment or distress, as manifested by 4-5 of the following, occurring within a 12-month period: 1) cocaine is often taken in larger amounts or over a longer period than was intended; 2) There is a persistent desire or unsuccessful efforts to cut down or control cocaine use; 3) A great deal of time is spent in activities necessary to obtain cocaine, use cocaine, or recover from its effects; 4) Craving, or a strong desire or urge to use cocaine; 5) Recurrent cocaine use resulting in a failure to fulfill major role obligations at work, school, or home; 6) Continued cocaine use despite having persistent or recurrent social or interpersonal problems caused or exacerbated by the effects of cocaine; 7) Important social, occupational, or recreational activities are given up or reduced because of cocaine use; 8) Recurrent cocaine use in situations in which it is physically hazardous; 9) cocaine use is continued despite knowledge of having a persistent or recurrent physical or psychological problem that is likely to have been caused or exacerbated by cocaine; 10) Tolerance, as defined by either of the following:a. A need for markedly increased amounts of cocaine to achieve intoxication or desired effect b. A markedly diminished effect with continued use of the same amount of cocaine; 11) Withdrawal, as manifested by either of the following: a. The characteristic withdrawal syndrome for cocaine. b. cocaine (or a closely related substance) is taken to relieve or avoid withdrawal symptoms." xsd:string
property_value: isDefinedBy "DSM_V" xsd:string

[Term]
id: 000162
name: DSM_V-defined severe cocaine use disorder
is_a: 000153 ! cocaine use disorder
property_value: dcterms:description "A problematic pattern of cocaine use leading to clinically significant impairment or distress, as manifested by six or more of the following, occurring within a 12-month period: 1) cocaine is often taken in larger amounts or over a longer period than was intended; 2) There is a persistent desire or unsuccessful efforts to cut down or control cocaine use; 3) A great deal of time is spent in activities necessary to obtain cocaine, use cocaine, or recover from its effects; 4) Craving, or a strong desire or urge to use cocaine; 5) Recurrent cocaine use resulting in a failure to fulfill major role obligations at work, school, or home; 6) Continued cocaine use despite having persistent or recurrent social or interpersonal problems caused or exacerbated by the effects of cocaine; 7) Important social, occupational, or recreational activities are given up or reduced because of cocaine use; 8) Recurrent cocaine use in situations in which it is physically hazardous; 9) cocaine use is continued despite knowledge of having a persistent or recurrent physical or psychological problem that is likely to have been caused or exacerbated by cocaine; 10) Tolerance, as defined by either of the following:a. A need for markedly increased amounts of cocaine to achieve intoxication or desired effect b. A markedly diminished effect with continued use of the same amount of cocaine; 11) Withdrawal, as manifested by either of the following: a. The characteristic withdrawal syndrome for cocaine. b. cocaine (or a closely related substance) is taken to relieve or avoid withdrawal symptoms." xsd:string
property_value: isDefinedBy "DSM_V" xsd:string

[Term]
id: 000163
name: recreational tobacco smoking
is_a: 000053 ! recreational nicotine use

[Term]
id: 000164
name: recreational vaping
is_a: 000053 ! recreational nicotine use

[Term]
id: 000165
name: non-repetitive binge tobacco smoking
is_a: 000052 ! non-repetitive binge nicotine use

[Term]
id: 000166
name: non-repetitive binge vaping
is_a: 000052 ! non-repetitive binge nicotine use

[Term]
id: 000167
name: chronic tobacco smoking
is_a: 000054 ! chronic nicotine use

[Term]
id: 000168
name: chronic vaping
is_a: 000054 ! chronic nicotine use

[Term]
id: 000169
name: heroin use
is_a: 000065 ! opioid use
property_value: dcterms:description "A substance use phenotype in which heroin is used. Use may be through inhalation, injection, ingestion or other means by which the substance may enter the body." xsd:string

[Term]
id: 000170
name: non-repetitive binge heroin use
is_a: 000006 ! non-repetitive binge substance use
is_a: 000169 ! heroin use
property_value: dcterms:description "A type of heroin use characterized by isolated or sporadic use of significant quantities of heroin in a short time period." xsd:string

[Term]
id: 000171
name: recreational heroin use
is_a: 000007 ! recreational substance use
is_a: 000169 ! heroin use
property_value: dcterms:description "A type of heroin use characterized by occasional limited use of heroin, without adverse consequences or behavioral/physiologic symptoms of a substance use disorder." xsd:string

[Term]
id: 000172
name: chronic heroin use
is_a: 000008 ! chronic substance use
is_a: 000169 ! heroin use
property_value: dcterms:description "A type of heroin use in which the use of heroin is frequent and persistent for a period of 3 months or greater; may or may not be accompanied by behavioral or physiologic symptoms necessary to define a substance use disorder." xsd:string

[Term]
id: 000173
name: heroin use disorder
is_a: 000172 ! chronic heroin use
property_value: dcterms:description "A type of chronic heroin use where there is continued use of heroin despite harm or adverse consequence to self or others. This is defined by behavioral criteria and physiologic symptoms." xsd:string

[Term]
id: 000174
name: heroin abuse
is_a: 000173 ! heroin use disorder
property_value: dcterms:description "A type of heroin use in which the amounts or methods of use of heroin are harmful or problematic to the individual or others (also called heroin misuse)" xsd:string

[Term]
id: 000175
name: DSM_IV-defined subsyndromic heroin abuse
is_a: 000174 ! heroin abuse
property_value: isDefinedBy "DSM_IV" xsd:string

[Term]
id: 000176
name: DSM_IV-defined syndromic heroin abuse
is_a: 000174 ! heroin abuse
property_value: dcterms:description "A maladaptive pattern of heroin use leading to clinically significant impairment or distress, as manifested by one (or more) of the following, occurring within a 12-month period: 1) Recurrent heroin use resulting in a failure to fulfill major role obligation at work, school, or home; 2) Recurrent heroin use in situations in which it is physically hazardous; 3) Recurrent heroin-related legal problems; 4) Continued heroin use despite having persistent or recurrent social or interpersonal problems caused or exacerbated by the effects of heroin." xsd:string
property_value: isDefinedBy "DSM_IV" xsd:string

[Term]
id: 000177
name: heroin dependence
is_a: 000173 ! heroin use disorder
property_value: dcterms:description "A type of heroin use in which the use of heroin is compulsive and repetitive and may result in tolerance to the effect of the drug and withdrawal symptoms when use is reduced or stopped." xsd:string

[Term]
id: 000178
name: DSM_IV-defined subsyndromic heroin dependence
is_a: 000177 ! heroin dependence
property_value: dcterms:description "A pattern of heroin use, leading to impairment or distress, as manifested by one to two of the following, occurring at any time in the same 12-month period: 1) Tolerance, as defined by either the following: a. Need for markedly increased amounts of heroin to achieve intoxication or desired effect. b. Markedly diminished effect with continued use of the same amount of heroin; 2) Withdrawal, as manifested by either of the following: a. The characteristic withdrawal syndrome for heroin. b. The same (or closely related) substance is taken to relieve or avoid withdrawal symptoms; 3) heroin is often taken in larger amounts or over a longer period than was intended; 4) There is persistent desire or unsuccessful efforts to cut down or control heroin use; 5) A great deal of time is spent in activities necessary to obtain heroin, use heroin or recover from its effects; 6) Important social, occupational, or recreational activities are given up or reduced because of heroin use; 7) heroin use is continued despite knowledge of having a persistent or recurrent physical or psychological problem that is likely to have been caused or exacerbated by heroin." xsd:string
property_value: isDefinedBy "DSM_IV" xsd:string

[Term]
id: 000179
name: DSM_IV-defined syndromic heroin dependence
is_a: 000177 ! heroin dependence
property_value: dcterms:description "A maladaptive pattern of heroin use, leading to significant impairment or distress, as manifested by three (or more) of the following, occurring at any time in the same 12-month period: 1) Tolerance, as defined by either the following: a. Need for markedly increased amounts of heroin to achieve intoxication or desired effect. b. Markedly diminished effect with continued use of the same amount of heroin; 2) Withdrawal, as manifested by either of the following: a. The characteristic withdrawal syndrome for heroin. b. The same (or closely related) substance is taken to relieve or avoid withdrawal symptoms; 3) heroin is often taken in larger amounts or over a longer period than was intended; 4) There is persistent desire or unsuccessful efforts to cut down or control heroin use; 5) A great deal of time is spent in activities necessary to obtain heroin, use heroin or recover from its effects; 6) Important social, occupational, or recreational activities are given up or reduced because of heroin use; 7) heroin use is continued despite knowledge of having a persistent or recurrent physical or psychological problem that is likely to have been caused or exacerbated by heroin." xsd:string
property_value: isDefinedBy "DSM_IV" xsd:string

[Term]
id: 000180
name: DSM_V-defined mild heroin use disorder
is_a: 000173 ! heroin use disorder
property_value: dcterms:description "A problematic pattern of heroin use leading to clinically significant impairment or distress, as manifested by two of the following, occurring within a 12-month period: 1) heroin is often taken in larger amounts or over a longer period than was intended; 2) There is a persistent desire or unsuccessful efforts to cut down or control heroin use; 3) A great deal of time is spent in activities necessary to obtain heroin, use heroin, or recover from its effects; 4) Craving, or a strong desire or urge to use heroin; 5) Recurrent heroin use resulting in a failure to fulfill major role obligations at work, school, or home; 6) Continued heroin use despite having persistent or recurrent social or interpersonal problems caused or exacerbated by the effects of heroin; 7) Important social, occupational, or recreational activities are given up or reduced because of heroin use; 8) Recurrent heroin use in situations in which it is physically hazardous; 9) heroin use is continued despite knowledge of having a persistent or recurrent physical or psychological problem that is likely to have been caused or exacerbated by heroin; 10) Tolerance, as defined by either of the following:a. A need for markedly increased amounts of heroin to achieve intoxication or desired effect b. A markedly diminished effect with continued use of the same amount of heroin; 11) Withdrawal, as manifested by either of the following: a. The characteristic withdrawal syndrome for heroin. b. heroin (or a closely related substance) is taken to relieve or avoid withdrawal symptoms." xsd:string
property_value: isDefinedBy "DSM_V" xsd:string

[Term]
id: 000181
name: DSM_V-defined moderate heroin use disorder
is_a: 000173 ! heroin use disorder
property_value: dcterms:description "A problematic pattern of heroin use leading to clinically significant impairment or distress, as manifested by 4-5 of the following, occurring within a 12-month period: 1) heroin is often taken in larger amounts or over a longer period than was intended; 2) There is a persistent desire or unsuccessful efforts to cut down or control heroin use; 3) A great deal of time is spent in activities necessary to obtain heroin, use heroin, or recover from its effects; 4) Craving, or a strong desire or urge to use heroin; 5) Recurrent heroin use resulting in a failure to fulfill major role obligations at work, school, or home; 6) Continued heroin use despite having persistent or recurrent social or interpersonal problems caused or exacerbated by the effects of heroin; 7) Important social, occupational, or recreational activities are given up or reduced because of heroin use; 8) Recurrent heroin use in situations in which it is physically hazardous; 9) heroin use is continued despite knowledge of having a persistent or recurrent physical or psychological problem that is likely to have been caused or exacerbated by heroin; 10) Tolerance, as defined by either of the following:a. A need for markedly increased amounts of heroin to achieve intoxication or desired effect b. A markedly diminished effect with continued use of the same amount of heroin; 11) Withdrawal, as manifested by either of the following: a. The characteristic withdrawal syndrome for heroin. b. heroin (or a closely related substance) is taken to relieve or avoid withdrawal symptoms." xsd:string
property_value: isDefinedBy "DSM_V" xsd:string

[Term]
id: 000182
name: DSM_V-defined severe heroin use disorder
is_a: 000173 ! heroin use disorder
property_value: dcterms:description "A problematic pattern of heroin use leading to clinically significant impairment or distress, as manifested by six or more of the following, occurring within a 12-month period: 1) heroin is often taken in larger amounts or over a longer period than was intended; 2) There is a persistent desire or unsuccessful efforts to cut down or control heroin use; 3) A great deal of time is spent in activities necessary to obtain heroin, use heroin, or recover from its effects; 4) Craving, or a strong desire or urge to use heroin; 5) Recurrent heroin use resulting in a failure to fulfill major role obligations at work, school, or home; 6) Continued heroin use despite having persistent or recurrent social or interpersonal problems caused or exacerbated by the effects of heroin; 7) Important social, occupational, or recreational activities are given up or reduced because of heroin use; 8) Recurrent heroin use in situations in which it is physically hazardous; 9) heroin use is continued despite knowledge of having a persistent or recurrent physical or psychological problem that is likely to have been caused or exacerbated by heroin; 10) Tolerance, as defined by either of the following:a. A need for markedly increased amounts of heroin to achieve intoxication or desired effect b. A markedly diminished effect with continued use of the same amount of heroin; 11) Withdrawal, as manifested by either of the following: a. The characteristic withdrawal syndrome for heroin. b. heroin (or a closely related substance) is taken to relieve or avoid withdrawal symptoms." xsd:string
property_value: isDefinedBy "DSM_V" xsd:string

[Term]
id: SUDO:0000000
name: root node

